Refactor wp-rules for IsPtr & Mov, and do a bit of cleanup wrt isFailWP

theories/rules/rules_IsPtr.v
@@ -16,132 +16,148 @@ Section cap_lang_rules.
   Implicit Types reg : gmap RegName Word.
   Implicit Types ms : gmap Addr Word.
 
-  Ltac inv_head_step :=
-    repeat match goal with
-           | _ => progress simplify_map_eq/= (* simplify memory stuff *)
-           | H : to_val _ = Some _ |- _ => apply of_to_val in H
-           | H : _ = of_val ?v |- _ =>
-             is_var v; destruct v; first[discriminate H|injection H as H]
-           | H : cap_lang.prim_step ?e _ _ _ _ _ |- _ =>
-             try (is_var e; fail 1); (* inversion yields many goals if [e] is a variable *)
-             (*    and can thus better be avoided. *)
-             let φ := fresh "φ" in 
-             inversion H as [| φ]; subst φ; clear H
-           end.
-
-  Ltac option_locate_mr m r :=
-    repeat match goal with
-           | H : m !! ?a = Some ?w |- _ => let Ha := fresh "H"a in
-                                         assert (m !m! a = w) as Ha; [ by (unfold MemLocate; rewrite H) | clear H]
-           | H : r !! ?a = Some ?w |- _ => let Ha := fresh "H"a in
-                                         assert (r !r! a = w) as Ha; [ by (unfold RegLocate; rewrite H) | clear H]
-           end.
-
-  Ltac inv_head_step_advanced m r HPC Hpc_a Hinstr Hstep Hpc_new1 :=
-    match goal with
-    | H : cap_lang.prim_step (Instr Executable) (r, m) _ ?e1 ?σ2 _ |- _ =>
-      let σ := fresh "σ" in
-      let e' := fresh "e'" in
-      let σ' := fresh "σ'" in
-      let Hstep' := fresh "Hstep'" in
-      let He0 := fresh "He0" in
-      let Ho := fresh "Ho" in
-      let He' := fresh "H"e' in
-      let Hσ' := fresh "H"σ' in
-      let Hefs := fresh "Hefs" in
-      let φ0 := fresh "φ" in
-      let p0 := fresh "p" in
-      let g0 := fresh "g" in
-      let b0 := fresh "b" in
-      let e2 := fresh "e" in
-      let a0 := fresh "a" in
-      let i := fresh "i" in
-      let c0 := fresh "c" in
-      let HregPC := fresh "HregPC" in
-      let Hi := fresh "H"i in
-      let Hexec := fresh "Hexec" in 
-      inversion Hstep as [ σ e' σ' Hstep' He0 Hσ Ho He' Hσ' Hefs |?|?|?]; 
-      inversion Hstep' as [φ0 | φ0 p0 g0 b0 e2 a0 i c0 HregPC ? Hi Hexec];
-      (simpl in *; try congruence );
-      subst e1 σ2 φ0 σ' e' σ; try subst c0; simpl in *;
-      try (rewrite HPC in HregPC;
-           inversion HregPC;
-           repeat match goal with
-                  | H : _ = p0 |- _ => destruct H
-                  | H : _ = g0 |- _ => destruct H
-                  | H : _ = b0 |- _ => destruct H
-                  | H : _ = e2 |- _ => destruct H
-                  | H : _ = a0 |- _ => destruct H
-                  end ; destruct Hi ; clear HregPC ;
-           rewrite Hpc_a Hinstr /= ;
-           rewrite Hpc_a Hinstr in Hstep)
+  Definition is_cap (w: Word): bool :=
+    match w with
+    | inr _ => true
+    | inl _ => false
     end.
 
   Inductive IsPtr_spec (regs: Reg) (dst src: RegName) (regs': Reg): cap_lang.val -> Prop :=
-  | IsPtr_spec_success:
-      incrementPC (<[ dst := match regs !! src with Some (inr _) => inl 1%Z | _ => inl 0%Z end]> regs) = Some regs' ->
+  | IsPtr_spec_success (w: Word):
+      regs !! src = Some w →
+      incrementPC (<[ dst := inl (if is_cap w then 1%Z else 0%Z) ]> regs) = Some regs' ->
       IsPtr_spec regs dst src regs' NextIV
-  | IsPtr_spec_failure:
+  | IsPtr_spec_failure (w: Word):
+      regs !! src = Some w →
+      incrementPC (<[ dst := inl (if is_cap w then 1%Z else 0%Z) ]> regs) = None ->
       IsPtr_spec regs dst src regs' FailedV.
-  
+
   Lemma wp_IsPtr Ep pc_p pc_g pc_b pc_e pc_a pc_p' w dst src regs :
     cap_lang.decode w = IsPtr dst src ->
-
     PermFlows pc_p pc_p' →
     isCorrectPC (inr ((pc_p, pc_g), pc_b, pc_e, pc_a)) →
     regs !! PC = Some (inr ((pc_p, pc_g), pc_b, pc_e, pc_a)) →
-    (∀ (ri: RegName), is_Some (regs !! ri)) →
+    regs_of (IsPtr dst src) ⊆ dom _ regs →
     {{{ ▷ pc_a ↦ₐ[pc_p'] w ∗
-          ▷ [∗ map] k↦y ∈ regs, k ↦ᵣ y }}}
+        ▷ [∗ map] k↦y ∈ regs, k ↦ᵣ y }}}
       Instr Executable @ Ep
     {{{ regs' retv, RET retv;
         ⌜ IsPtr_spec regs dst src regs' retv ⌝ ∗
           pc_a ↦ₐ[pc_p'] w ∗
           [∗ map] k↦y ∈ regs', k ↦ᵣ y }}}.
   Proof.
-    iIntros (Hinstr Hfl Hvpc HPC Hri φ) "(>Hpc_a & >Hmap) Hφ".
+    iIntros (Hinstr Hfl Hvpc HPC Dregs φ) "(>Hpc_a & >Hmap) Hφ".
     iApply wp_lift_atomic_head_step_no_fork; auto.
     iIntros (σ1 l1 l2 n) "Hσ1 /=". destruct σ1; simpl.
     iDestruct "Hσ1" as "[Hr Hm]".
     assert (pc_p' ≠ O).
     { destruct pc_p'; auto. destruct pc_p; inversion Hfl.
       inversion Hvpc; subst; destruct H7 as [Hcontr | [Hcontr | Hcontr]]; inversion Hcontr. }
-    pose proof (regs_lookup_eq _ _ _ HPC) as HPC'.
-    iAssert (⌜ r = regs ⌝)%I with "[Hr Hmap]" as %->.
-    { iApply (gen_heap_valid_allSepM with "[Hr]"); eauto. }
+    iDestruct (gen_heap_valid_inclSepM with "Hr Hmap") as %Hregs.
+    have HPC' := regs_lookup_eq _ _ _ HPC.
+    have ? := lookup_weaken _ _ _ _ HPC Hregs.
     iDestruct (@gen_heap_valid_cap with "Hm Hpc_a") as %Hpc_a; auto.
-    (*option_locate_mr m r.*) iModIntro.
-    iSplitR. by iPureIntro; apply normal_always_head_reducible.
+    iModIntro. iSplitR. by iPureIntro; apply normal_always_head_reducible.
     iNext. iIntros (e2 σ2 efs Hpstep).
     apply prim_step_exec_inv in Hpstep as (-> & -> & (c & -> & Hstep)).
     iSplitR; auto. eapply step_exec_inv in Hstep; eauto.
-    
-    destruct (Hri src) as [wsrc Hsrc].
-    destruct (incrementPC (<[ dst := match wsrc with inl _ => inl 0%Z | inr _ => inl 1%Z end ]> regs)) as [regs'|] eqn:Hregs'; cycle 1.
-    { assert (c = Failed /\ σ2 = ((<[ dst := match wsrc with inl _ => inl 0%Z | inr _ => inl 1%Z end ]> regs), m)) as (-> & ->).
-      { cbn in Hstep. rewrite /RegLocate Hsrc in Hstep.
-        destruct wsrc; rewrite (incrementPC_fail_updatePC _ _ Hregs') in Hstep; inv Hstep; auto. }
-      iMod ((gen_heap_update_inSepM _ _ dst) with "Hr Hmap") as "[Hr Hmap]"; eauto.
-      iFrame. iApply "Hφ"; iFrame.
-      iPureIntro. econstructor 2. }
 
-    cbn in Hstep. rewrite /RegLocate Hsrc in Hstep.
-    assert ((c, σ2) = updatePC (update_reg (regs, m) dst (match wsrc with inl _ => inl 0%Z | inr _ => inl 1%Z end))) as HH.
-    { destruct wsrc; auto. }
+    specialize (indom_regs_incl _ _ _ Dregs Hregs) as Hri. unfold regs_of in Hri.
+    destruct (Hri dst) as [wdst [H'dst Hdst]]. by set_solver+.
+    destruct (Hri src) as [wsrc [H'src Hsrc]]. by set_solver+.
+
+    destruct (incrementPC (<[ dst := inl (if is_cap wsrc then 1%Z else 0%Z) ]> regs))
+      as [regs'|] eqn:Hregs'; pose proof Hregs' as H'regs'; cycle 1.
+    { apply incrementPC_fail_updatePC with (m:=m) in Hregs'.
+      eapply updatePC_fail_incl with (m':=m) in Hregs'.
+      2: by apply lookup_insert_is_Some'; eauto.
+      2: by apply insert_mono; eauto.
+      assert (c = Failed /\ σ2 = ((<[ dst := inl (if is_cap wsrc then 1%Z else 0%Z) ]> r), m)) as (-> & ->).
+      { rewrite /= /RegLocate /update_reg Hsrc /= in Hstep. unfold is_cap in Hregs' |- *.
+        destruct wsrc; simplify_pair_eq; eauto. }
+      iMod ((gen_heap_update_inSepM _ _ dst) with "Hr Hmap") as "[Hr Hmap]"; eauto.
+      iFrame. iApply "Hφ"; iFrame. iPureIntro. econstructor; eauto. }
+
+    (* Success *)
+
+    rewrite /= /RegLocate Hsrc in Hstep.
+    assert ((c, σ2) = updatePC (update_reg (r, m) dst (inl (if is_cap wsrc then 1%Z else 0%Z)))) as HH.
+    { unfold is_cap; destruct wsrc; auto. }
 
     eapply (incrementPC_success_updatePC _ m) in Hregs'
       as (p' & g' & b' & e' & a'' & a_pc' & HPC'' & Ha_pc' & HuPC & ->).
-    rewrite HuPC in HH; clear HuPC; inversion HH; clear HH; subst c σ2. cbn.
-    iFrame.
+    eapply updatePC_success_incl with (m':=m) in HuPC. 2: by eapply insert_mono; eauto.
+    rewrite HuPC in HH. simplify_eq. iFrame.
     iMod ((gen_heap_update_inSepM _ _ dst) with "Hr Hmap") as "[Hr Hmap]"; eauto.
     iMod ((gen_heap_update_inSepM _ _ PC) with "Hr Hmap") as "[Hr Hmap]"; eauto.
-    iFrame. iModIntro. iApply "Hφ". iFrame. iPureIntro.
-    econstructor 1; eauto.
-    by rewrite Hsrc /incrementPC HPC'' Ha_pc'.
+    iFrame. iModIntro. iApply "Hφ". iFrame. iPureIntro. econstructor; eauto.
   Qed.
 
-   Lemma wp_IsPtr_successPC E pc_p pc_g pc_b pc_e pc_a pc_a' w dst w' pc_p' :
-     cap_lang.decode w = IsPtr dst PC →
+  Lemma wp_IsPtr_successPC E pc_p pc_g pc_b pc_e pc_a pc_a' w dst w' pc_p' :
+    cap_lang.decode w = IsPtr dst PC →
+    PermFlows pc_p pc_p' → isCorrectPC (inr ((pc_p,pc_g),pc_b,pc_e,pc_a)) →
+    (pc_a + 1)%a = Some pc_a' →
+    dst ≠ PC →
+
+    {{{ ▷ PC ↦ᵣ inr ((pc_p,pc_g),pc_b,pc_e,pc_a)
+        ∗ ▷ pc_a ↦ₐ[pc_p'] w
+        ∗ ▷ dst ↦ᵣ w'
+    }}}
+      Instr Executable @ E
+      {{{ RET NextIV;
+          PC ↦ᵣ inr ((pc_p,pc_g),pc_b,pc_e,pc_a')
+          ∗ pc_a ↦ₐ[pc_p'] w
+          ∗ dst ↦ᵣ inl 1%Z }}}.
+   Proof.
+     iIntros (Hinstr Hfl Hvpc Hpca' Hne ϕ) "(>HPC & >Hpc_a & >Hdst) Hφ".
+     iDestruct (map_of_regs_2 with "HPC Hdst") as "[Hmap %]".
+     iApply (wp_IsPtr with "[$Hmap Hpc_a]"); eauto; simplify_map_eq; eauto.
+     by rewrite !dom_insert; set_solver+.
+     iNext. iIntros (regs' retv) "(#Hspec & Hpc_a & Hmap)". iDestruct "Hspec" as %Hspec.
+
+     destruct Hspec as [|].
+     { iApply "Hφ". iFrame. incrementPC_inv; simplify_map_eq.
+       rewrite (insert_commute _ PC dst) // insert_insert insert_commute // insert_insert.
+       iDestruct (regs_of_map_2 with "Hmap") as "(?&?)"; eauto; iFrame. }
+     { incrementPC_inv; simplify_map_eq; eauto. congruence. }
+   Qed.
+
+   Lemma wp_IsPtr_success E pc_p pc_g pc_b pc_e pc_a pc_a' w dst r wr w' pc_p' :
+     cap_lang.decode w = IsPtr dst r →
+     PermFlows pc_p pc_p' → isCorrectPC (inr ((pc_p,pc_g),pc_b,pc_e,pc_a)) →
+     (pc_a + 1)%a = Some pc_a' →
+     dst ≠ PC →
+
+       {{{ ▷ PC ↦ᵣ inr ((pc_p,pc_g),pc_b,pc_e,pc_a)
+             ∗ ▷ pc_a ↦ₐ[pc_p'] w
+             ∗ ▷ r ↦ᵣ wr
+             ∗ ▷ dst ↦ᵣ w'
+       }}}
+         Instr Executable @ E
+       {{{ RET NextIV;
+           PC ↦ᵣ inr ((pc_p,pc_g),pc_b,pc_e,pc_a')
+           ∗ pc_a ↦ₐ[pc_p'] w
+           ∗ r ↦ᵣ wr
+           ∗ dst ↦ᵣ inl (if is_cap wr then 1%Z else 0%Z) }}}.
+   Proof.
+    iIntros (Hinstr Hfl Hvpc Hpc_a Hdst ϕ) "(>HPC & >Hpc_a & >Hr & >Hdst) Hφ".
+    iDestruct (map_of_regs_3 with "HPC Hr Hdst") as "[Hmap (%&%&%)]".
+    iApply (wp_IsPtr with "[$Hmap Hpc_a]"); eauto; simplify_map_eq; eauto.
+    by rewrite !dom_insert; set_solver+.
+    iNext. iIntros (regs' retv) "(#Hspec & Hpc_a & Hmap)". iDestruct "Hspec" as %Hspec.
+
+    destruct Hspec as [|].
+    { (* Success *)
+      iApply "Hφ". iFrame. incrementPC_inv; simplify_map_eq.
+      rewrite (insert_commute _ PC dst) // insert_insert (insert_commute _ r dst) //
+              (insert_commute _ dst PC) // insert_insert.
+      iDestruct (regs_of_map_3 with "Hmap") as "(?&?&?)"; eauto; iFrame. }
+    { (* Failure (contradiction) *)
+      incrementPC_inv; simplify_map_eq; eauto. congruence. }
+   Qed.
+
+   Lemma wp_IsPtr_success_dst E pc_p pc_g pc_b pc_e pc_a pc_a' w dst w' pc_p' :
+     cap_lang.decode w = IsPtr dst dst →
      PermFlows pc_p pc_p' → isCorrectPC (inr ((pc_p,pc_g),pc_b,pc_e,pc_a)) →
      (pc_a + 1)%a = Some pc_a' →
      dst ≠ PC →
@@ -154,345 +170,19 @@ Section cap_lang_rules.
        {{{ RET NextIV;
            PC ↦ᵣ inr ((pc_p,pc_g),pc_b,pc_e,pc_a')
            ∗ pc_a ↦ₐ[pc_p'] w
-           ∗ dst ↦ᵣ inl 1%Z }}}.
+           ∗ dst ↦ᵣ inl (if is_cap w' then 1%Z else 0%Z) }}}.
    Proof.
-     iIntros (Hinstr Hfl Hvpc Hpca' Hne ϕ) "(>HPC & >Hpc_a & >Hdst) Hϕ".
-     iApply wp_lift_atomic_head_step_no_fork; auto.
-     iIntros (σ1 l1 l2 n) "Hσ1 /=". destruct σ1; simpl.
-     iDestruct "Hσ1" as "[Hr0 Hm]".
-    assert (pc_p' ≠ O) as Ho.
-    { destruct pc_p'; auto. destruct pc_p; inversion Hfl.
-      inversion Hvpc; subst;
-        destruct H7 as [Hcontr | [Hcontr | Hcontr]]; inversion Hcontr. }
-     iDestruct (@gen_heap_valid_cap with "Hm Hpc_a") as %?; auto. 
-     iDestruct (@gen_heap_valid with "Hr0 HPC") as %?.
-     iDestruct (@gen_heap_valid with "Hr0 Hdst") as %?.
-     option_locate_mr m r0.
-     assert (HPC: r !r! PC = inr (pc_p, pc_g, pc_b, pc_e, pc_a)) by (unfold RegLocate; rewrite H2; auto).
-     assert (<[dst:=inl 1%Z]> r !r! PC = (inr (pc_p, pc_g, pc_b, pc_e, pc_a))) as Hpc_new1.
-     { rewrite (locate_ne_reg _ _ _ (inr (pc_p, pc_g, pc_b, pc_e, pc_a))); eauto. }
-     iApply fupd_frame_l.
-     iSplit.
-     - rewrite /reducible.
-       iExists [], (Instr _),(<[PC:=inr (pc_p, pc_g, pc_b, pc_e, pc_a')]> (<[dst:=inl 1%Z]> r), m), [].
-       iPureIntro.
-       constructor.
-       apply (step_exec_instr (r,m) pc_p pc_g pc_b pc_e pc_a
-                              (IsPtr dst PC)
-                              (NextI,_)); eauto; simpl; try congruence.
-       by rewrite HPC /update_reg /updatePC /= Hpc_new1 Hpca' /update_reg /updatePC /=.
-     - (*iMod (fupd_intro_mask' ⊤) as "H"; eauto.*)
-       iModIntro. iNext.
-       iIntros (e1 σ2 efs Hstep).
-       inv_head_step_advanced m r HPC Hpc_a Hinstr Hstep Hpc_new1.
-       rewrite HPC /updatePC /update_reg /= Hpc_new1 Hpca' /=.
-       iMod (@gen_heap_update with "Hr0 Hdst") as "[Hr0 Hdst]".
-       iMod (@gen_heap_update with "Hr0 HPC") as "[$ HPC]".
-       iSpecialize ("Hϕ" with "[HPC Hdst Hpc_a]"); iFrame.
-       iModIntro. done.
-   Qed.
+     iIntros (Hinstr Hfl Hvpc Hpca' Hne ϕ) "(>HPC & >Hpc_a & >Hdst) Hφ".
+     iDestruct (map_of_regs_2 with "HPC Hdst") as "[Hmap %]".
+     iApply (wp_IsPtr with "[$Hmap Hpc_a]"); eauto; simplify_map_eq; eauto.
+     by rewrite !dom_insert; set_solver+.
+     iNext. iIntros (regs' retv) "(#Hspec & Hpc_a & Hmap)". iDestruct "Hspec" as %Hspec.
 
-   Lemma wp_IsPtr_success E pc_p pc_g pc_b pc_e pc_a pc_a' w dst r wr w' pc_p' :
-     cap_lang.decode w = IsPtr dst r →
-     PermFlows pc_p pc_p' → isCorrectPC (inr ((pc_p,pc_g),pc_b,pc_e,pc_a)) →
-     (pc_a + 1)%a = Some pc_a' →
-     dst ≠ PC →
-
-       {{{ ▷ PC ↦ᵣ inr ((pc_p,pc_g),pc_b,pc_e,pc_a)
-             ∗ ▷ pc_a ↦ₐ[pc_p'] w
-             ∗ if reg_eq_dec r dst then ▷ r ↦ᵣ wr else ▷ r ↦ᵣ wr ∗ ▷ dst ↦ᵣ w'
-       }}}
-         Instr Executable @ E
-       {{{ RET NextIV;
-           PC ↦ᵣ inr ((pc_p,pc_g),pc_b,pc_e,pc_a')
-           ∗ pc_a ↦ₐ[pc_p'] w
-           ∗ if reg_eq_dec r dst then r ↦ᵣ inl (match wr with inr _ => 1%Z | inl _ => 0%Z end) else r ↦ᵣ wr ∗ dst ↦ᵣ inl (match wr with inr _ => 1%Z | inl _ => 0%Z end) }}}.
-   Proof.
-     destruct (reg_eq_dec r dst). 
-     { subst dst.
-       iIntros (Hinstr Hfl Hvpc Hpca' Hne ϕ) "(>HPC & >Hpc_a & >Hr) Hϕ".
-       iApply wp_lift_atomic_head_step_no_fork; auto.
-       iIntros (σ1 l1 l2 n) "Hσ1 /=". destruct σ1; simpl.
-       iDestruct "Hσ1" as "[Hr0 Hm]".
-    assert (pc_p' ≠ O) as Ho.
-    { destruct pc_p'; auto. destruct pc_p; inversion Hfl.
-      inversion Hvpc; subst;
-        destruct H7 as [Hcontr | [Hcontr | Hcontr]]; inversion Hcontr. }
-       iDestruct (@gen_heap_valid_cap with "Hm Hpc_a") as %?; auto. 
-       iDestruct (@gen_heap_valid with "Hr0 HPC") as %?.
-       iDestruct (@gen_heap_valid with "Hr0 Hr") as %?.
-       option_locate_mr m r0.
-       assert (<[r:=inl (match wr with inr _ => 1%Z | inl _ => 0%Z end)]> r0 !r! PC = (inr (pc_p, pc_g, pc_b, pc_e, pc_a))) as Hpc_new1.
-       { rewrite (locate_ne_reg _ _ _ (inr (pc_p, pc_g, pc_b, pc_e, pc_a))); eauto. }
-       iApply fupd_frame_l.
-       iSplit.
-       - rewrite /reducible.
-         iExists [], (Instr _),(<[PC:=inr (pc_p, pc_g, pc_b, pc_e, pc_a')]> (<[r:=inl (match wr with inr _ => 1%Z | inl _ => 0%Z end)]> r0), m), [].
-         iPureIntro.
-         constructor.
-         apply (step_exec_instr (r0,m) pc_p pc_g pc_b pc_e pc_a
-                                (IsPtr r r)
-                                (NextI,_)); eauto; simpl; try congruence.
-         destruct wr; by rewrite Hr /update_reg /updatePC /= Hpc_new1 Hpca' /update_reg /updatePC /=.
-       - (*iMod (fupd_intro_mask' ⊤) as "H"; eauto.*)
-         iModIntro. iNext.
-         iIntros (e1 σ2 efs Hstep).
-         inv_head_step_advanced m r0 HPC Hpc_a Hinstr Hstep Hpc_new1.
-         destruct wr; rewrite Hr /updatePC /update_reg /= Hpc_new1 Hpca' /=.
-         iMod (@gen_heap_update with "Hr0 Hr") as "[Hr0 Hdst]".
-         iMod (@gen_heap_update with "Hr0 HPC") as "[$ HPC]".
-         iSpecialize ("Hϕ" with "[HPC Hdst Hpc_a]"); iFrame.
-         iModIntro. done.
-         iMod (@gen_heap_update with "Hr0 Hr") as "[Hr0 Hdst]".
-         iMod (@gen_heap_update with "Hr0 HPC") as "[$ HPC]".
-         iSpecialize ("Hϕ" with "[HPC Hdst Hpc_a]"); iFrame.
-         iModIntro. done. }
-     { clear n.
-       iIntros (Hinstr Hfl Hvpc Hpca' Hne ϕ) "(>HPC & >Hpc_a & >Hr & >Hdst) Hϕ".
-       iApply wp_lift_atomic_head_step_no_fork; auto.
-       iIntros (σ1 l1 l2 n) "Hσ1 /=". destruct σ1; simpl.
-       iDestruct "Hσ1" as "[Hr0 Hm]".
-    assert (pc_p' ≠ O) as Ho.
-    { destruct pc_p'; auto. destruct pc_p; inversion Hfl.
-      inversion Hvpc; subst;
-        destruct H7 as [Hcontr | [Hcontr | Hcontr]]; inversion Hcontr. }
-       iDestruct (@gen_heap_valid_cap with "Hm Hpc_a") as %?; auto. 
-       iDestruct (@gen_heap_valid with "Hr0 HPC") as %?.
-       iDestruct (@gen_heap_valid with "Hr0 Hr") as %?.
-       iDestruct (@gen_heap_valid with "Hr0 Hdst") as %?.
-       option_locate_mr m r0.
-       assert (<[dst:=inl (match wr with inr _ => 1%Z | inl _ => 0%Z end)]> r0 !r! PC = (inr (pc_p, pc_g, pc_b, pc_e, pc_a))) as Hpc_new1.
-       { rewrite (locate_ne_reg _ _ _ (inr (pc_p, pc_g, pc_b, pc_e, pc_a))); eauto. }
-       iApply fupd_frame_l.
-       iSplit.
-       - rewrite /reducible.
-         iExists [], (Instr _),(<[PC:=inr (pc_p, pc_g, pc_b, pc_e, pc_a')]> (<[dst:=inl (match wr with inr _ => 1%Z | inl _ => 0%Z end)]> r0), m), [].
-         iPureIntro.
-         constructor.
-         apply (step_exec_instr (r0,m) pc_p pc_g pc_b pc_e pc_a
-                                (IsPtr dst r)
-                                (NextI,_)); eauto; simpl; try congruence.
-         destruct wr; by rewrite Hr /update_reg /updatePC /= Hpc_new1 Hpca' /update_reg /updatePC /=.
-       - (*iMod (fupd_intro_mask' ⊤) as "H"; eauto.*)
-         iModIntro. iNext.
-         iIntros (e1 σ2 efs Hstep).
-         inv_head_step_advanced m r0 HPC Hpc_a Hinstr Hstep Hpc_new1.
-         destruct wr; rewrite Hr /updatePC /update_reg /= Hpc_new1 Hpca' /=.
-         iMod (@gen_heap_update with "Hr0 Hdst") as "[Hr0 Hdst]".
-         iMod (@gen_heap_update with "Hr0 HPC") as "[$ HPC]".
-         iSpecialize ("Hϕ" with "[HPC Hdst Hpc_a Hr]"); iFrame.
-         iModIntro. done.
-         iMod (@gen_heap_update with "Hr0 Hdst") as "[Hr0 Hdst]".
-         iMod (@gen_heap_update with "Hr0 HPC") as "[$ HPC]".
-         iSpecialize ("Hϕ" with "[HPC Hdst Hpc_a Hr]"); iFrame.
-         iModIntro. done. }
-   Qed.
-
-   Lemma wp_IsPtr_fail_PC E pc_p pc_g pc_b pc_e pc_a w src w' pc_p' :
-     cap_lang.decode w = IsPtr PC src →
-     PermFlows pc_p pc_p' → isCorrectPC (inr ((pc_p,pc_g),pc_b,pc_e,pc_a)) →
-
-     {{{ (if reg_eq_dec PC src then
-            ▷ PC ↦ᵣ inr ((pc_p,pc_g),pc_b,pc_e,pc_a) else
-            ▷ PC ↦ᵣ inr ((pc_p,pc_g),pc_b,pc_e,pc_a) ∗ ▷ src ↦ᵣ w')
-          ∗ ▷ pc_a ↦ₐ[pc_p'] w
-       }}}
-         Instr Executable @ E
-       {{{ RET FailedV;
-           (if reg_eq_dec PC src then PC ↦ᵣ inl 1%Z else PC ↦ᵣ inl match w' with inl _ => 0%Z | _ => 1%Z end ∗ src ↦ᵣ w') 
-           ∗ pc_a ↦ₐ[pc_p'] w }}}.
-   Proof.
-     destruct (reg_eq_dec PC src).
-     - subst src.
-       intros Hinstr Hfl Hvpc.
-       iIntros (ϕ) "(>HPC & >Hpc_a) Hϕ".
-       iApply wp_lift_atomic_head_step_no_fork; auto.
-       iIntros (σ1 l1 l2 n) "Hσ1 /=". destruct σ1; simpl.
-       iDestruct "Hσ1" as "[Hr0 Hm]".
-    assert (pc_p' ≠ O) as Ho.
-    { destruct pc_p'; auto. destruct pc_p; inversion Hfl.
-      inversion Hvpc; subst;
-        destruct H7 as [Hcontr | [Hcontr | Hcontr]]; inversion Hcontr. }
-       iDestruct (@gen_heap_valid_cap with "Hm Hpc_a") as %?; auto. 
-       iDestruct (@gen_heap_valid with "Hr0 HPC") as %?.
-       option_locate_mr m r.
-       iApply fupd_frame_l.
-       iSplit.
-       + rewrite /reducible.
-         iExists [], (Instr _), _, [].
-         iPureIntro.
-         constructor.
-         eapply (step_exec_instr (r,m) pc_p pc_g pc_b pc_e pc_a
-                                (IsPtr PC PC)
-                                (Failed,_)); eauto; simpl; try (unfold RegLocate; rewrite H2; auto); try congruence.
-         rewrite HPC /update_reg /updatePC /= /RegLocate lookup_insert. auto.
-       + iModIntro. iNext.
-         iIntros (e1 σ2 efs Hstep).
-         inv_head_step_advanced m r HPC Hpc_a Hinstr Hstep HPC.
-         rewrite HPC. rewrite /updatePC /update_reg /RegLocate lookup_insert /=.
-         iMod (@gen_heap_update with "Hr0 HPC") as "[Hr0 HPC]".
-         iSpecialize ("Hϕ" with "[HPC Hpc_a]"); iFrame.
-         iModIntro. done.
-     - rename n into Hn.
-       intros Hinstr Hfl Hvpc.
-       iIntros (ϕ) "((>HPC & >Hsrc) & >Hpc_a) Hϕ".
-       iApply wp_lift_atomic_head_step_no_fork; auto.
-       iIntros (σ1 l1 l2 n) "Hσ1 /=". destruct σ1; simpl.
-       iDestruct "Hσ1" as "[Hr Hm]".
-    assert (pc_p' ≠ O) as Ho.
-    { destruct pc_p'; auto. destruct pc_p; inversion Hfl.
-      inversion Hvpc; subst;
-        destruct H7 as [Hcontr | [Hcontr | Hcontr]]; inversion Hcontr. }
-       iDestruct (@gen_heap_valid_cap with "Hm Hpc_a") as %?; auto. 
-       iDestruct (@gen_heap_valid with "Hr HPC") as %?.
-       iDestruct (@gen_heap_valid with "Hr Hsrc") as %?.
-       option_locate_mr m r.
-       iApply fupd_frame_l.
-       iSplit.
-       + rewrite /reducible.
-         iExists [], (Instr _), _, [].
-         iPureIntro.
-         constructor.
-         eapply (step_exec_instr (r,m) pc_p pc_g pc_b pc_e pc_a
-                                (IsPtr PC src)
-                                (Failed, (<[PC:=inl match w' with inl _ => 0%Z | inr _ => 1%Z end]> r, m))); eauto; simpl; try congruence.
-         rewrite Hsrc /update_reg /updatePC /= /RegLocate lookup_insert. destruct w'; auto.
-         rewrite lookup_insert; auto.
-       + iModIntro. iNext.
-         iIntros (e1 σ2 efs Hstep).
-         inv_head_step_advanced m r HPC Hpc_a Hinstr Hstep HPC.
-         rewrite Hsrc. rewrite /updatePC /update_reg /RegLocate lookup_insert /=.
-         iMod (@gen_heap_update with "Hr HPC") as "[Hr0 HPC]".
-         iSpecialize ("Hϕ" with "[HPC Hsrc Hpc_a]"); iFrame.
-         iModIntro. rewrite lookup_insert. destruct w'; simpl; iFrame; done.
-   Qed.
-
-   Lemma wp_IsPtr_fail E pc_p pc_g pc_b pc_e pc_a w dst r wr w' pc_p' :
-     cap_lang.decode w = IsPtr dst r →
-     PermFlows pc_p pc_p' → isCorrectPC (inr ((pc_p,pc_g),pc_b,pc_e,pc_a)) →
-     (pc_a + 1)%a = None →
-     dst ≠ PC →
-
-       {{{ ▷ PC ↦ᵣ inr ((pc_p,pc_g),pc_b,pc_e,pc_a)
-             ∗ ▷ pc_a ↦ₐ[pc_p'] w
-             ∗ if reg_eq_dec r dst then ▷ r ↦ᵣ wr else
-                 if reg_eq_dec r PC then ▷ dst ↦ᵣ w' else ▷ r ↦ᵣ wr ∗ ▷ dst ↦ᵣ w'
-       }}}
-         Instr Executable @ E
-       {{{ RET FailedV;
-           PC ↦ᵣ inr ((pc_p,pc_g),pc_b,pc_e,pc_a)
-           ∗ pc_a ↦ₐ[pc_p'] w
-           ∗ if reg_eq_dec r dst then r ↦ᵣ inl (match wr with inr _ => 1%Z | inl _ => 0%Z end) else
-               if reg_eq_dec r PC then dst ↦ᵣ inl 1%Z else r ↦ᵣ wr ∗ dst ↦ᵣ inl (match wr with inr _ => 1%Z | inl _ => 0%Z end) }}}.
-   Proof.
-     destruct (reg_eq_dec r dst). 
-     { subst dst.
-       iIntros (Hinstr Hfl Hvpc Hpca' Hne ϕ) "(>HPC & >Hpc_a & >Hr) Hϕ".
-       iApply wp_lift_atomic_head_step_no_fork; auto.
-       iIntros (σ1 l1 l2 n) "Hσ1 /=". destruct σ1; simpl.
-       iDestruct "Hσ1" as "[Hr0 Hm]".
-    assert (pc_p' ≠ O) as Ho.
-    { destruct pc_p'; auto. destruct pc_p; inversion Hfl.
-      inversion Hvpc; subst;
-        destruct H7 as [Hcontr | [Hcontr | Hcontr]]; inversion Hcontr. }
-       iDestruct (@gen_heap_valid_cap with "Hm Hpc_a") as %?; auto. 
-       iDestruct (@gen_heap_valid with "Hr0 HPC") as %?.
-       iDestruct (@gen_heap_valid with "Hr0 Hr") as %?.
-       option_locate_mr m r0.
-       assert (<[r:=inl (match wr with inr _ => 1%Z | inl _ => 0%Z end)]> r0 !r! PC = (inr (pc_p, pc_g, pc_b, pc_e, pc_a))) as Hpc_new1.
-       { rewrite (locate_ne_reg _ _ _ (inr (pc_p, pc_g, pc_b, pc_e, pc_a))); eauto. }
-       iApply fupd_frame_l.
-       iSplit.
-       - rewrite /reducible.
-         iExists [], (Instr _), (<[r:=inl (match wr with inr _ => 1%Z | inl _ => 0%Z end)]> r0, m), [].
-         iPureIntro.
-         constructor.
-         apply (step_exec_instr (r0,m) pc_p pc_g pc_b pc_e pc_a
-                                (IsPtr r r)
-                                (Failed,_)); eauto; simpl; try congruence.
-         destruct wr; by rewrite Hr /update_reg /updatePC /= Hpc_new1 Hpca' /update_reg /updatePC /=.
-       - (*iMod (fupd_intro_mask' ⊤) as "H"; eauto.*)
-         iModIntro. iNext.
-         iIntros (e1 σ2 efs Hstep).
-         inv_head_step_advanced m r0 HPC Hpc_a Hinstr Hstep Hpc_new1.
-         destruct wr; rewrite Hr /updatePC /update_reg /= Hpc_new1 Hpca' /=.
-         iMod (@gen_heap_update with "Hr0 Hr") as "[Hr0 Hdst]".
-         iSpecialize ("Hϕ" with "[HPC Hdst Hpc_a]"); iFrame.
-         iModIntro. done.
-         iMod (@gen_heap_update with "Hr0 Hr") as "[Hr0 Hdst]".
-         iSpecialize ("Hϕ" with "[HPC Hdst Hpc_a]"); iFrame.
-         iModIntro. done. }
-     { rename n into Hn. destruct (reg_eq_dec r PC).
-       { subst r.
-         iIntros (Hinstr Hfl Hvpc Hpca' Hne ϕ) "(>HPC & >Hpc_a & >Hdst) Hϕ".
-         iApply wp_lift_atomic_head_step_no_fork; auto.
-         iIntros (σ1 l1 l2 n) "Hσ1 /=". destruct σ1; simpl.
-         iDestruct "Hσ1" as "[Hr0 Hm]".
-    assert (pc_p' ≠ O) as Ho.
-    { destruct pc_p'; auto. destruct pc_p; inversion Hfl.
-      inversion Hvpc; subst;
-        destruct H7 as [Hcontr | [Hcontr | Hcontr]]; inversion Hcontr. }
-         iDestruct (@gen_heap_valid_cap with "Hm Hpc_a") as %?; auto. 
-         iDestruct (@gen_heap_valid with "Hr0 HPC") as %?.
-         iDestruct (@gen_heap_valid with "Hr0 Hdst") as %?.
-         option_locate_mr m r.
-         assert (<[dst:=inl 1%Z]> r !r! PC = (inr (pc_p, pc_g, pc_b, pc_e, pc_a))) as Hpc_new1.
-         { rewrite (locate_ne_reg _ _ _ (inr (pc_p, pc_g, pc_b, pc_e, pc_a))); eauto. }
-         iApply fupd_frame_l.
-         iSplit.
-         - rewrite /reducible.
-           iExists [], (Instr _),(<[dst:=inl 1%Z]> r, m), [].
-           iPureIntro.
-           constructor.
-           apply (step_exec_instr (r,m) pc_p pc_g pc_b pc_e pc_a
-                                  (IsPtr dst PC)
-                                  (Failed,_)); eauto; simpl; try congruence.
-           by rewrite HPC /update_reg /updatePC /= Hpc_new1 Hpca' /update_reg /updatePC /=.
-         - (*iMod (fupd_intro_mask' ⊤) as "H"; eauto.*)
-           iModIntro. iNext.
-           iIntros (e1 σ2 efs Hstep).
-           inv_head_step_advanced m r HPC Hpc_a Hinstr Hstep Hpc_new1.
-           rewrite HPC /updatePC /update_reg /= Hpc_new1 Hpca' /=.
-           iMod (@gen_heap_update with "Hr0 Hdst") as "[Hr0 Hdst]".
-           iSpecialize ("Hϕ" with "[HPC Hdst Hpc_a]"); iFrame.
-           iModIntro. done. }
-       { clear n.
-         iIntros (Hinstr Hfl Hvpc Hpca' Hne ϕ) "(>HPC & >Hpc_a & >Hr & >Hdst) Hϕ".
-         iApply wp_lift_atomic_head_step_no_fork; auto.
-         iIntros (σ1 l1 l2 n) "Hσ1 /=". destruct σ1; simpl.
-         iDestruct "Hσ1" as "[Hr0 Hm]". 
-    assert (pc_p' ≠ O) as Ho.
-    { destruct pc_p'; auto. destruct pc_p; inversion Hfl.
-      inversion Hvpc; subst;
-        destruct H7 as [Hcontr | [Hcontr | Hcontr]]; inversion Hcontr. }
-         iDestruct (@gen_heap_valid_cap with "Hm Hpc_a") as %?; auto. 
-         iDestruct (@gen_heap_valid with "Hr0 HPC") as %?.
-         iDestruct (@gen_heap_valid with "Hr0 Hr") as %?.
-         iDestruct (@gen_heap_valid with "Hr0 Hdst") as %?.
-         option_locate_mr m r0.
-         assert (<[dst:=inl (match wr with inr _ => 1%Z | inl _ => 0%Z end)]> r0 !r! PC = (inr (pc_p, pc_g, pc_b, pc_e, pc_a))) as Hpc_new1.
-         { rewrite (locate_ne_reg _ _ _ (inr (pc_p, pc_g, pc_b, pc_e, pc_a))); eauto. }
-         iApply fupd_frame_l.
-         iSplit.
-         - rewrite /reducible.
-           iExists [], (Instr _),(<[dst:=inl (match wr with inr _ => 1%Z | inl _ => 0%Z end)]> r0, m), [].
-           iPureIntro.
-           constructor.
-           apply (step_exec_instr (r0,m) pc_p pc_g pc_b pc_e pc_a
-                                  (IsPtr dst r)
-                                  (Failed,_)); eauto; simpl; try congruence.
-           destruct wr; by rewrite Hr /update_reg /updatePC /= Hpc_new1 Hpca' /update_reg /updatePC /=.
-         - (*iMod (fupd_intro_mask' ⊤) as "H"; eauto.*)
-           iModIntro. iNext.
-           iIntros (e1 σ2 efs Hstep).
-           inv_head_step_advanced m r0 HPC Hpc_a Hinstr Hstep Hpc_new1.
-           destruct wr; rewrite Hr /updatePC /update_reg /= Hpc_new1 Hpca' /=.
-           iMod (@gen_heap_update with "Hr0 Hdst") as "[Hr0 Hdst]".
-           iSpecialize ("Hϕ" with "[HPC Hdst Hpc_a Hr]"); iFrame.
-           iModIntro. done.
-           iMod (@gen_heap_update with "Hr0 Hdst") as "[Hr0 Hdst]".
-           iSpecialize ("Hϕ" with "[HPC Hdst Hpc_a Hr]"); iFrame.
-           iModIntro. done. } }
+     destruct Hspec as [|].
+     { iApply "Hφ". iFrame. incrementPC_inv; simplify_map_eq.
+       rewrite (insert_commute _ PC dst) // insert_insert insert_commute // insert_insert.
+       iDestruct (regs_of_map_2 with "Hmap") as "(?&?)"; eauto; iFrame. }
+     { incrementPC_inv; simplify_map_eq; eauto. congruence. }
    Qed.
 
 End cap_lang_rules.
