theories/rules/rules_Mov.v
@@ -16,135 +16,81 @@ Section cap_lang_rules.
   Implicit Types reg : gmap RegName Word.
   Implicit Types ms : gmap Addr Word.
 
-  Ltac inv_head_step :=
-    repeat match goal with
-           | _ => progress simplify_map_eq/= (* simplify memory stuff *)
-           | H : to_val _ = Some _ |- _ => apply of_to_val in H
-           | H : _ = of_val ?v |- _ =>
-             is_var v; destruct v; first[discriminate H|injection H as H]
-           | H : cap_lang.prim_step ?e _ _ _ _ _ |- _ =>
-             try (is_var e; fail 1); (* inversion yields many goals if [e] is a variable *)
-             (*    and can thus better be avoided. *)
-             let φ := fresh "φ" in 
-             inversion H as [| φ]; subst φ; clear H
-           end.
-
-  Ltac option_locate_mr m r :=
-    repeat match goal with
-           | H : m !! ?a = Some ?w |- _ => let Ha := fresh "H"a in
-                                         assert (m !m! a = w) as Ha; [ by (unfold MemLocate; rewrite H) | clear H]
-           | H : r !! ?a = Some ?w |- _ => let Ha := fresh "H"a in
-                                         assert (r !r! a = w) as Ha; [ by (unfold RegLocate; rewrite H) | clear H]
-           end.
-
-  Ltac inv_head_step_advanced m r HPC Hpc_a Hinstr Hstep Hpc_new1 :=
-    match goal with
-    | H : cap_lang.prim_step (Instr Executable) (r, m) _ ?e1 ?σ2 _ |- _ =>
-      let σ := fresh "σ" in
-      let e' := fresh "e'" in
-      let σ' := fresh "σ'" in
-      let Hstep' := fresh "Hstep'" in
-      let He0 := fresh "He0" in
-      let Ho := fresh "Ho" in
-      let He' := fresh "H"e' in
-      let Hσ' := fresh "H"σ' in
-      let Hefs := fresh "Hefs" in
-      let φ0 := fresh "φ" in
-      let p0 := fresh "p" in
-      let g0 := fresh "g" in
-      let b0 := fresh "b" in
-      let e2 := fresh "e" in
-      let a0 := fresh "a" in
-      let i := fresh "i" in
-      let c0 := fresh "c" in
-      let HregPC := fresh "HregPC" in
-      let Hi := fresh "H"i in
-      let Hexec := fresh "Hexec" in 
-      inversion Hstep as [ σ e' σ' Hstep' He0 Hσ Ho He' Hσ' Hefs |?|?|?]; 
-      inversion Hstep' as [φ0 | φ0 p0 g0 b0 e2 a0 i c0 HregPC ? Hi Hexec];
-      (simpl in *; try congruence );
-      subst e1 σ2 φ0 σ' e' σ; try subst c0; simpl in *;
-      try (rewrite HPC in HregPC;
-           inversion HregPC;
-           repeat match goal with
-                  | H : _ = p0 |- _ => destruct H
-                  | H : _ = g0 |- _ => destruct H
-                  | H : _ = b0 |- _ => destruct H
-                  | H : _ = e2 |- _ => destruct H
-                  | H : _ = a0 |- _ => destruct H
-                  end ; destruct Hi ; clear HregPC ;
-           rewrite Hpc_a Hinstr /= ;
-           rewrite Hpc_a Hinstr in Hstep)
-    end.
-
-  (* TODO: Move to rules_base.v *)
-  Definition word_of_argument (regs: Reg) (a: Z + RegName): option Word :=
-    match a with
-    | inl n => Some (inl n)
-    | inr r => regs !! r
-    end.
-
   Inductive Mov_spec (regs: Reg) (dst: RegName) (src: Z + RegName) (regs': Reg): cap_lang.val -> Prop :=
   | IsPtr_spec_success w:
-      word_of_argument regs src = Some w ->
-      incrementPC (<[ dst := w]> regs) = Some regs' ->
+      word_of_argument regs src = Some w →
+      incrementPC (<[ dst := w ]> regs) = Some regs' →
       Mov_spec regs dst src regs' NextIV
-  | Mov_spec_failure:
+  | Mov_spec_failure w:
+      word_of_argument regs src = Some w →
+      incrementPC (<[ dst := w ]> regs) = None →
       Mov_spec regs dst src regs' FailedV.
 
   Lemma wp_Mov Ep pc_p pc_g pc_b pc_e pc_a pc_p' w dst src regs :
     cap_lang.decode w = Mov dst src ->
-
     PermFlows pc_p pc_p' →
     isCorrectPC (inr ((pc_p, pc_g), pc_b, pc_e, pc_a)) →
     regs !! PC = Some (inr ((pc_p, pc_g), pc_b, pc_e, pc_a)) →
-    (∀ (ri: RegName), is_Some (regs !! ri)) →
+    regs_of (Mov dst src) ⊆ dom _ regs →
     {{{ ▷ pc_a ↦ₐ[pc_p'] w ∗
-          ▷ [∗ map] k↦y ∈ regs, k ↦ᵣ y }}}
+        ▷ [∗ map] k↦y ∈ regs, k ↦ᵣ y }}}
       Instr Executable @ Ep
     {{{ regs' retv, RET retv;
         ⌜ Mov_spec regs dst src regs' retv ⌝ ∗
-          pc_a ↦ₐ[pc_p'] w ∗
-          [∗ map] k↦y ∈ regs', k ↦ᵣ y }}}.
+        pc_a ↦ₐ[pc_p'] w ∗
+        [∗ map] k↦y ∈ regs', k ↦ᵣ y }}}.
   Proof.
-    iIntros (Hinstr Hfl Hvpc HPC Hri φ) "(>Hpc_a & >Hmap) Hφ".
+    iIntros (Hinstr Hfl Hvpc HPC Dregs φ) "(>Hpc_a & >Hmap) Hφ".
     iApply wp_lift_atomic_head_step_no_fork; auto.
     iIntros (σ1 l1 l2 n) "Hσ1 /=". destruct σ1; simpl.
     iDestruct "Hσ1" as "[Hr Hm]".
     assert (pc_p' ≠ O).
     { destruct pc_p'; auto. destruct pc_p; inversion Hfl.
       inversion Hvpc; subst; destruct H7 as [Hcontr | [Hcontr | Hcontr]]; inversion Hcontr. }
-    pose proof (regs_lookup_eq _ _ _ HPC) as HPC'.
-    iAssert (⌜ r = regs ⌝)%I with "[Hr Hmap]" as %->.
-    { iApply (gen_heap_valid_allSepM with "[Hr]"); eauto. }
+    iDestruct (gen_heap_valid_inclSepM with "Hr Hmap") as %Hregs.
+    have HPC' := regs_lookup_eq _ _ _ HPC.
+    have ? := lookup_weaken _ _ _ _ HPC Hregs.
     iDestruct (@gen_heap_valid_cap with "Hm Hpc_a") as %Hpc_a; auto.
-    (*option_locate_mr m r.*) iModIntro.
-    iSplitR. by iPureIntro; apply normal_always_head_reducible.
+    iModIntro. iSplitR. by iPureIntro; apply normal_always_head_reducible.
     iNext. iIntros (e2 σ2 efs Hpstep).
     apply prim_step_exec_inv in Hpstep as (-> & -> & (c & -> & Hstep)).
     iSplitR; auto. eapply step_exec_inv in Hstep; eauto.
 
-    assert (exists w, word_of_argument regs src = Some w) as [wsrc Hwsrc].
-    { destruct src; eauto.
-      destruct (Hri r). eauto. }
-    destruct (incrementPC (<[ dst := wsrc ]> regs)) as [regs'|] eqn:Hregs'; cycle 1.
-    { assert (c = Failed /\ σ2 = ((<[ dst := wsrc ]> regs), m)) as (-> & ->).
-      { cbn in Hstep. destruct src; simpl in Hwsrc; [inv Hwsrc | rewrite /RegLocate Hwsrc in Hstep]; rewrite (incrementPC_fail_updatePC _ _ Hregs') in Hstep; inv Hstep; auto. }
-      iMod ((gen_heap_update_inSepM _ _ dst) with "Hr Hmap") as "[Hr Hmap]"; eauto.
-      iFrame. iApply "Hφ"; iFrame.
-      iPureIntro. econstructor 2. }
+    specialize (indom_regs_incl _ _ _ Dregs Hregs) as Hri. unfold regs_of in Hri.
+    destruct (Hri dst) as [wdst [H'dst Hdst]]. by set_solver+.
 
-    cbn in Hstep. assert ((c, σ2) = updatePC (update_reg (regs, m) dst wsrc)) as HH.
-    { destruct src; simpl in Hwsrc; [inv Hwsrc | rewrite /RegLocate Hwsrc in Hstep]; auto. }
+    assert (exists w, word_of_argument regs src = Some w) as [wsrc Hwsrc].
+    { destruct src as [| r0]; eauto; cbn.
+      destruct (Hri r0) as [? [? ?]]. set_solver+. eauto. }
+
+    pose proof Hwsrc as Hwsrc'. eapply word_of_argument_Some_inv' in Hwsrc; eauto.
+
+    destruct (incrementPC (<[ dst := wsrc ]> regs)) as [regs'|] eqn:Hregs';
+      pose proof Hregs' as H'regs'; cycle 1.
+    { apply incrementPC_fail_updatePC with (m:=m) in Hregs'.
+      eapply updatePC_fail_incl with (m':=m) in Hregs'.
+      2: by apply lookup_insert_is_Some'; eauto.
+      2: by apply insert_mono; eauto.
+
+      assert (c = Failed /\ σ2 = ((<[ dst := wsrc ]> r), m)) as (-> & ->).
+      { destruct Hwsrc as [ [? [? ?] ] | [? (? & ? & Hr') ] ].
+        all: rewrite /= /update_reg /RegLocate /= in Hstep; simplify_pair_eq; eauto.
+        rewrite Hr' /= in Hstep. by simplify_pair_eq. }
+      iMod ((gen_heap_update_inSepM _ _ dst) with "Hr Hmap") as "[Hr Hmap]"; eauto.
+      iFrame. iApply "Hφ"; iFrame. iPureIntro. econstructor; eauto. }
+
+    rewrite /= /RegLocate in Hstep.
+    assert ((c, σ2) = updatePC (update_reg (r, m) dst wsrc)) as HH.
+    { destruct Hwsrc as [ [? [? ?] ] | [? (? & ? & Hr') ] ]; simplify_eq; eauto.
+      by rewrite Hr' in Hstep. }
+    rewrite /update_reg /= in HH.
     eapply (incrementPC_success_updatePC _ m) in Hregs'
       as (p' & g' & b' & e' & a'' & a_pc' & HPC'' & Ha_pc' & HuPC & ->).
-    rewrite HuPC in HH; clear HuPC; inversion HH; clear HH; subst c σ2. cbn.
-    iFrame.
+    eapply updatePC_success_incl with (m':=m) in HuPC. 2: by eapply insert_mono; eauto.
+    rewrite HuPC in HH; simplify_eq. iFrame.
     iMod ((gen_heap_update_inSepM _ _ dst) with "Hr Hmap") as "[Hr Hmap]"; eauto.
     iMod ((gen_heap_update_inSepM _ _ PC) with "Hr Hmap") as "[Hr Hmap]"; eauto.
-    iFrame. iModIntro. iApply "Hφ". iFrame. iPureIntro.
-    econstructor 1; eauto.
-    by rewrite /incrementPC HPC'' Ha_pc'.
+    iFrame. iModIntro. iApply "Hφ". iFrame. iPureIntro. econstructor; eauto.
   Qed.
 
   Lemma wp_move_success_z E pc_p pc_g pc_b pc_e pc_a pc_a' w r1 wr1 z pc_p' :
@@ -155,46 +101,27 @@ Section cap_lang_rules.
     PC ≠ r1 →
 
     {{{ ▷ PC ↦ᵣ inr ((pc_p,pc_g),pc_b,pc_e,pc_a)
-          ∗ ▷ pc_a ↦ₐ[pc_p'] w
-          ∗ ▷ r1 ↦ᵣ wr1 }}}
+        ∗ ▷ pc_a ↦ₐ[pc_p'] w
+        ∗ ▷ r1 ↦ᵣ wr1 }}}
       Instr Executable @ E
       {{{ RET NextIV;
           PC ↦ᵣ inr ((pc_p,pc_g),pc_b,pc_e,pc_a')
-             ∗ pc_a ↦ₐ[pc_p'] w
-             ∗ r1 ↦ᵣ inl z }}}.
+          ∗ pc_a ↦ₐ[pc_p'] w
+          ∗ r1 ↦ᵣ inl z }}}.
   Proof.
-    iIntros (Hinstr Hfl Hvpc Hpca' Hne ϕ) "(>HPC & >Hpc_a & >Hr1) Hϕ".
-    iApply wp_lift_atomic_head_step_no_fork; auto.
-    iIntros (σ1 l1 l2 n) "Hσ1 /=". destruct σ1; simpl.
-    iDestruct "Hσ1" as "[Hr Hm]".
-    assert (pc_p' ≠ O).
-    { destruct pc_p'; auto. destruct pc_p; inversion Hfl. inversion Hvpc; subst;
-      destruct H7 as [Hcontr | [Hcontr | Hcontr]]; inversion Hcontr. }
-    iDestruct (@gen_heap_valid with "Hr HPC") as %?.
-    iDestruct (@gen_heap_valid_cap with "Hm Hpc_a") as %?; auto. 
-    iDestruct (@gen_heap_valid with "Hr Hr1") as %?.
-    option_locate_mr m r.
-    assert (<[r1:=inl z]> r !r! PC = (inr (pc_p, pc_g, pc_b, pc_e, pc_a)))
-      as Hpc_new1.
-    { rewrite (locate_ne_reg _ _ _ (inr (pc_p, pc_g, pc_b, pc_e, pc_a))); eauto. } 
-    iApply fupd_frame_l.
-    iSplit.
-    - rewrite /reducible.
-      iExists [], (Instr _),(updatePC (update_reg (r,m) r1 (inl z))).2, [].
-      iPureIntro.
-      constructor.
-      apply (step_exec_instr (r,m) pc_p pc_g pc_b pc_e pc_a
-                             (Mov r1 (inl z))
-                             (NextI,_)); eauto; simpl; try congruence.
-        by rewrite /updatePC /update_reg /= Hpc_new1 Hpca'.  
-    - (*iMod (fupd_intro_mask' ⊤) as "H"; eauto.*)
-      iModIntro. iNext.
-      iIntros (e1 σ2 efs Hstep).
-      inv_head_step_advanced m r HPC Hpc_a Hinstr Hstep Hpc_new1.
-      rewrite /updatePC /update_reg /= Hpc_new1 Hpca' /=.  
-      iMod (@gen_heap_update with "Hr Hr1") as "[Hr Hr1]". 
-      iMod (@gen_heap_update with "Hr HPC") as "[$ HPC]". 
-      iSpecialize ("Hϕ" with "[HPC Hr1 Hpc_a]"); iFrame; eauto.
+    iIntros (Hinstr Hfl Hvpc Hpca' Hne ϕ) "(>HPC & >Hpc_a & >Hr1) Hφ".
+    iDestruct (map_of_regs_2 with "HPC Hr1") as "[Hmap %]".
+    iApply (wp_Mov with "[$Hmap Hpc_a]"); eauto; simplify_map_eq; eauto.
+    by unfold regs_of; rewrite !dom_insert; set_solver+.
+    iNext. iIntros (regs' retv) "(#Hspec & Hpc_a & Hmap)". iDestruct "Hspec" as %Hspec.
+
+    destruct Hspec as [|].
+    { (* Success *)
+      iApply "Hφ". iFrame. incrementPC_inv; simplify_map_eq.
+      rewrite (insert_commute _ PC r1) // insert_insert insert_commute // insert_insert.
+      iDestruct (regs_of_map_2 with "Hmap") as "(?&?)"; eauto; iFrame. }
+    { (* Failure (contradiction) *)
+      incrementPC_inv; simplify_map_eq; eauto. congruence. }
   Qed.
 
   Lemma wp_move_success_reg E pc_p pc_g pc_b pc_e pc_a pc_a' w r1 wr1 rv wrv pc_p' :
@@ -205,49 +132,29 @@ Section cap_lang_rules.
     PC ≠ r1 →
 
     {{{ ▷ PC ↦ᵣ inr ((pc_p,pc_g),pc_b,pc_e,pc_a)
-          ∗ ▷ pc_a ↦ₐ[pc_p'] w
-          ∗ ▷ r1 ↦ᵣ wr1
-          ∗ ▷ rv ↦ᵣ wrv }}}
+        ∗ ▷ pc_a ↦ₐ[pc_p'] w
+        ∗ ▷ r1 ↦ᵣ wr1
+        ∗ ▷ rv ↦ᵣ wrv }}}
       Instr Executable @ E
       {{{ RET NextIV;
           PC ↦ᵣ inr ((pc_p,pc_g),pc_b,pc_e,pc_a')
-             ∗ pc_a ↦ₐ[pc_p'] w
-             ∗ r1 ↦ᵣ wrv
-             ∗ rv ↦ᵣ wrv }}}.
+          ∗ pc_a ↦ₐ[pc_p'] w
+          ∗ r1 ↦ᵣ wrv
+          ∗ rv ↦ᵣ wrv }}}.
   Proof.
-    iIntros (Hinstr Hfl Hvpc Hpca' Hne ϕ) "(>HPC & >Hpc_a & >Hr1 & >Hrv) Hϕ".
-    iApply wp_lift_atomic_head_step_no_fork; auto.
-    iIntros (σ1 l1 l2 n) "Hσ1 /=". destruct σ1; simpl.
-    iDestruct "Hσ1" as "[Hr Hm]".
-    assert (pc_p' ≠ O).
-    { destruct pc_p'; auto. destruct pc_p; inversion Hfl. inversion Hvpc; subst;
-      destruct H7 as [Hcontr | [Hcontr | Hcontr]]; inversion Hcontr. }
-    iDestruct (@gen_heap_valid with "Hr HPC") as %?.
-    iDestruct (@gen_heap_valid_cap with "Hm Hpc_a") as %?; auto. 
-    iDestruct (@gen_heap_valid with "Hr Hr1") as %?.
-    iDestruct (@gen_heap_valid with "Hr Hrv") as %?.
-    option_locate_mr m r.
-    assert (<[r1:=wrv]> r !r! PC = (inr (pc_p, pc_g, pc_b, pc_e, pc_a)))
-      as Hpc_new1.
-    { rewrite (locate_ne_reg _ _ _ (inr (pc_p, pc_g, pc_b, pc_e, pc_a))); eauto. } 
-    iApply fupd_frame_l.
-    iSplit.
-    - rewrite /reducible.
-      iExists [], (Instr _),(updatePC (update_reg (r,m) r1 wrv)).2, [].
-      iPureIntro.
-      constructor.
-      apply (step_exec_instr (r,m) pc_p pc_g pc_b pc_e pc_a
-                             (Mov r1 (inr rv))
-                             (NextI,_)); eauto; simpl; try congruence.
-        by rewrite /updatePC /update_reg /= Hrv Hpc_new1 Hpca'.  
-    - (*iMod (fupd_intro_mask' ⊤) as "H"; eauto.*)
-      iModIntro. iNext.
-      iIntros (e1 σ2 efs Hstep).
-      inv_head_step_advanced m r HPC Hpc_a Hinstr Hstep Hpc_new1.
-      rewrite /updatePC /update_reg /= Hrv Hpc_new1 Hpca' /=.  
-      iMod (@gen_heap_update with "Hr Hr1") as "[Hr Hr1]". 
-      iMod (@gen_heap_update with "Hr HPC") as "[$ HPC]". 
-      iSpecialize ("Hϕ" with "[HPC Hr1 Hpc_a Hrv]"); iFrame; eauto.
+    iIntros (Hinstr Hfl Hvpc Hpca' Hne ϕ) "(>HPC & >Hpc_a & >Hr1 & >Hrv) Hφ".
+    iDestruct (map_of_regs_3 with "HPC Hr1 Hrv") as "[Hmap (%&%&%)]".
+    iApply (wp_Mov with "[$Hmap Hpc_a]"); eauto; simplify_map_eq; eauto.
+    by unfold regs_of; rewrite !dom_insert; set_solver+.
+    iNext. iIntros (regs' retv) "(#Hspec & Hpc_a & Hmap)". iDestruct "Hspec" as %Hspec.
+
+    destruct Hspec as [|].
+    { (* Success *)
+      iApply "Hφ". iFrame. incrementPC_inv; simplify_map_eq.
+      rewrite (insert_commute _ PC r1) // insert_insert (insert_commute _ PC r1) // insert_insert.
+      iDestruct (regs_of_map_3 with "Hmap") as "(?&?&?)"; eauto; iFrame. }
+    { (* Failure (contradiction) *)
+      incrementPC_inv; simplify_map_eq; eauto. congruence. }
   Qed.
 
   Lemma wp_move_success_reg_same E pc_p pc_g pc_b pc_e pc_a pc_a' w r1 wr1 pc_p' :
@@ -258,46 +165,27 @@ Section cap_lang_rules.
     PC ≠ r1 →
 
     {{{ ▷ PC ↦ᵣ inr ((pc_p,pc_g),pc_b,pc_e,pc_a)
-          ∗ ▷ pc_a ↦ₐ[pc_p'] w
-          ∗ ▷ r1 ↦ᵣ wr1 }}}
+        ∗ ▷ pc_a ↦ₐ[pc_p'] w
+        ∗ ▷ r1 ↦ᵣ wr1 }}}
       Instr Executable @ E
       {{{ RET NextIV;
           PC ↦ᵣ inr ((pc_p,pc_g),pc_b,pc_e,pc_a')
-             ∗ pc_a ↦ₐ[pc_p'] w
-             ∗ r1 ↦ᵣ wr1 }}}.
+          ∗ pc_a ↦ₐ[pc_p'] w
+          ∗ r1 ↦ᵣ wr1 }}}.
   Proof.
-    iIntros (Hinstr Hfl Hvpc Hpca' Hne ϕ) "(>HPC & >Hpc_a & >Hr1) Hϕ".
-    iApply wp_lift_atomic_head_step_no_fork; auto.
-    iIntros (σ1 l1 l2 n) "Hσ1 /=". destruct σ1; simpl.
-    iDestruct "Hσ1" as "[Hr Hm]".
-    assert (pc_p' ≠ O).
-    { destruct pc_p'; auto. destruct pc_p; inversion Hfl. inversion Hvpc; subst;
-      destruct H7 as [Hcontr | [Hcontr | Hcontr]]; inversion Hcontr. }
-    iDestruct (@gen_heap_valid with "Hr HPC") as %?.
-    iDestruct (@gen_heap_valid_cap with "Hm Hpc_a") as %?; auto. 
-    iDestruct (@gen_heap_valid with "Hr Hr1") as %?.
-    option_locate_mr m r.
-    assert (<[r1:=wr1]> r !r! PC = (inr (pc_p, pc_g, pc_b, pc_e, pc_a)))
-      as Hpc_new1.
-    { rewrite (locate_ne_reg _ _ _ (inr (pc_p, pc_g, pc_b, pc_e, pc_a))); eauto. } 
-    iApply fupd_frame_l.
-    iSplit.
-    - rewrite /reducible.
-      iExists [], (Instr _),(updatePC (update_reg (r,m) r1 wr1)).2, [].
-      iPureIntro.
-      constructor.
-      apply (step_exec_instr (r,m) pc_p pc_g pc_b pc_e pc_a
-                             (Mov r1 (inr r1))
-                             (NextI,_)); eauto; simpl; try congruence.
-        by rewrite /updatePC /update_reg /= Hr1 Hpc_new1 Hpca'.  
-    - (*iMod (fupd_intro_mask' ⊤) as "H"; eauto.*)
-      iModIntro. iNext.
-      iIntros (e1 σ2 efs Hstep).
-      inv_head_step_advanced m r HPC Hpc_a Hinstr Hstep Hpc_new1.
-      rewrite /updatePC /update_reg /= Hr1 Hpc_new1 Hpca' /=.  
-      iMod (@gen_heap_update with "Hr Hr1") as "[Hr Hr1]". 
-      iMod (@gen_heap_update with "Hr HPC") as "[$ HPC]".
-      iSpecialize ("Hϕ" with "[HPC Hr1 Hpc_a]"); iFrame; eauto.
+    iIntros (Hinstr Hfl Hvpc Hpca' Hne ϕ) "(>HPC & >Hpc_a & >Hr1) Hφ".
+    iDestruct (map_of_regs_2 with "HPC Hr1") as "[Hmap %]".
+    iApply (wp_Mov with "[$Hmap Hpc_a]"); eauto; simplify_map_eq; eauto.
+    by unfold regs_of; rewrite !dom_insert; set_solver+.
+    iNext. iIntros (regs' retv) "(#Hspec & Hpc_a & Hmap)". iDestruct "Hspec" as %Hspec.
+
+    destruct Hspec as [|].
+    { (* Success *)
+      iApply "Hφ". iFrame. incrementPC_inv; simplify_map_eq.
+      rewrite (insert_commute _ PC r1) // insert_insert insert_commute // insert_insert.
+      iDestruct (regs_of_map_2 with "Hmap") as "(?&?)"; eauto; iFrame. }
+    { (* Failure (contradiction) *)
+      incrementPC_inv; simplify_map_eq; eauto. congruence. }
   Qed.
 
   Lemma wp_move_success_reg_samePC E pc_p pc_g pc_b pc_e pc_a pc_a' w pc_p' :
@@ -307,42 +195,25 @@ Section cap_lang_rules.
     (pc_a + 1)%a = Some pc_a' →
 
     {{{ ▷ PC ↦ᵣ inr ((pc_p,pc_g),pc_b,pc_e,pc_a)
-          ∗ ▷ pc_a ↦ₐ[pc_p'] w }}}
+        ∗ ▷ pc_a ↦ₐ[pc_p'] w }}}
       Instr Executable @ E
       {{{ RET NextIV;
           PC ↦ᵣ inr ((pc_p,pc_g),pc_b,pc_e,pc_a')
-             ∗ pc_a ↦ₐ[pc_p'] w }}}.
+          ∗ pc_a ↦ₐ[pc_p'] w }}}.
   Proof.
-    iIntros (Hinstr Hfl Hvpc Hpca' ϕ) "(>HPC & >Hpc_a) Hϕ".
-    iApply wp_lift_atomic_head_step_no_fork; auto.
-    iIntros (σ1 l1 l2 n) "Hσ1 /=". destruct σ1; simpl.
-    iDestruct "Hσ1" as "[Hr Hm]".
-    assert (pc_p' ≠ O).
-    { destruct pc_p'; auto. destruct pc_p; inversion Hfl. inversion Hvpc; subst;
-      destruct H7 as [Hcontr | [Hcontr | Hcontr]]; inversion Hcontr. }
-    iDestruct (@gen_heap_valid with "Hr HPC") as %?.
-    iDestruct (@gen_heap_valid_cap with "Hm Hpc_a") as %?; auto. 
-    option_locate_mr m r.
-    iApply fupd_frame_l.
-    iSplit.
-    - rewrite /reducible.
-      iExists [], (Instr _),_, [].
-      iPureIntro.
-      constructor.
-      eapply (step_exec_instr (r,m) pc_p pc_g pc_b pc_e pc_a
-                              (Mov PC (inr PC))
-                              (_,_)); eauto; simpl; try congruence.
-      rewrite /updatePC /update_reg /= /RegLocate lookup_insert.
-      rewrite /RegLocate in HPC. rewrite HPC Hpca'. eauto.
-    - (*iMod (fupd_intro_mask' ⊤) as "H"; eauto.*)
-      iModIntro. iNext.
-      iIntros (e1 σ2 efs Hstep).
-      inv_head_step_advanced m r HPC Hpc_a Hinstr Hstep HPC.
-      rewrite /updatePC /update_reg /= /RegLocate lookup_insert.
-      rewrite /RegLocate in HPC. rewrite HPC Hpca' /=.
-      rewrite insert_insert.
-      iMod (@gen_heap_update with "Hr HPC") as "[$ HPC]".
-      iSpecialize ("Hϕ" with "[HPC Hpc_a]"); iFrame; eauto.
+    iIntros (Hinstr Hfl Hvpc Hpca' ϕ) "(>HPC & >Hpc_a) Hφ".
+    iDestruct (map_of_regs_1 with "HPC") as "Hmap".
+    iApply (wp_Mov with "[$Hmap Hpc_a]"); eauto; simplify_map_eq; eauto.
+    by unfold regs_of; rewrite !dom_insert; set_solver+.
+    iNext. iIntros (regs' retv) "(#Hspec & Hpc_a & Hmap)". iDestruct "Hspec" as %Hspec.
+
+    destruct Hspec as [|].
+    { (* Success *)
+      iApply "Hφ". iFrame. incrementPC_inv; simplify_map_eq.
+      rewrite !insert_insert.
+      iDestruct (regs_of_map_1 with "Hmap") as "?"; eauto; iFrame. }
+    { (* Failure (contradiction) *)
+      incrementPC_inv; simplify_map_eq; eauto. congruence. }
   Qed.
 
   Lemma wp_move_success_reg_toPC E pc_p pc_g pc_b pc_e pc_a w r1 p g b e a a' pc_p' :
@@ -352,43 +223,27 @@ Section cap_lang_rules.
     (a + 1)%a = Some a' →
 
     {{{ ▷ PC ↦ᵣ inr ((pc_p,pc_g),pc_b,pc_e,pc_a)
-          ∗ ▷ pc_a ↦ₐ[pc_p'] w
-          ∗ ▷ r1 ↦ᵣ inr ((p,g),b,e,a) }}}
+        ∗ ▷ pc_a ↦ₐ[pc_p'] w
+        ∗ ▷ r1 ↦ᵣ inr ((p,g),b,e,a) }}}
       Instr Executable @ E
       {{{ RET NextIV;
           PC ↦ᵣ inr ((p,g),b,e,a')
-             ∗ pc_a ↦ₐ[pc_p'] w
-             ∗ r1 ↦ᵣ inr ((p,g),b,e,a) }}}.
+          ∗ pc_a ↦ₐ[pc_p'] w
+          ∗ r1 ↦ᵣ inr ((p,g),b,e,a) }}}.
   Proof.
-    iIntros (Hinstr Hfl Hvpc Hpca' ϕ) "(>HPC & >Hpc_a & >Hr1) Hϕ".
-    iApply wp_lift_atomic_head_step_no_fork; auto.
-    iIntros (σ1 l1 l2 n) "Hσ1 /=". destruct σ1; simpl.
-    iDestruct "Hσ1" as "[Hr Hm]".
-    assert (pc_p' ≠ O).
-    { destruct pc_p'; auto. destruct pc_p; inversion Hfl. inversion Hvpc; subst;
-      destruct H7 as [Hcontr | [Hcontr | Hcontr]]; inversion Hcontr. }
-    iDestruct (@gen_heap_valid with "Hr HPC") as %?.
-    iDestruct (@gen_heap_valid_cap with "Hm Hpc_a") as %?; auto. 
-    iDestruct (@gen_heap_valid with "Hr Hr1") as %?.
-    option_locate_mr m r.
-    iApply fupd_frame_l.
-    iSplit.
-    - rewrite /reducible.
-      iExists [], (Instr _),_, [].
-      iPureIntro.
-      constructor.
-      eapply (step_exec_instr (r,m) pc_p pc_g pc_b pc_e pc_a
-                              (Mov PC (inr r1))
-                              (NextI,_)); eauto; simpl; try congruence.
-        by rewrite /updatePC /update_reg /= Hr1 /RegLocate lookup_insert Hpca'.
-    - (*iMod (fupd_intro_mask' ⊤) as "H"; eauto.*)
-      iModIntro. iNext.
-      iIntros (e1 σ2 efs Hstep).
-      inv_head_step_advanced m r HPC Hpc_a Hinstr Hstep Hpc_new1.
-      rewrite /updatePC /update_reg /= Hr1 /RegLocate lookup_insert Hpca' /=.
-      rewrite insert_insert.
-      iMod (@gen_heap_update with "Hr HPC") as "[$ HPC]".
-      iSpecialize ("Hϕ" with "[HPC Hr1 Hpc_a]"); iFrame; eauto.
+    iIntros (Hinstr Hfl Hvpc Hpca' ϕ) "(>HPC & >Hpc_a & >Hr1) Hφ".
+    iDestruct (map_of_regs_2 with "HPC Hr1") as "[Hmap %]".
+    iApply (wp_Mov with "[$Hmap Hpc_a]"); eauto; simplify_map_eq; eauto.
+    by unfold regs_of; rewrite !dom_insert; set_solver+.
+    iNext. iIntros (regs' retv) "(#Hspec & Hpc_a & Hmap)". iDestruct "Hspec" as %Hspec.
+
+    destruct Hspec as [|].
+    { (* Success *)
+      iApply "Hφ". iFrame. incrementPC_inv; simplify_map_eq.
+      rewrite (insert_commute _ PC r1) // insert_insert insert_commute // insert_insert.
+      iDestruct (regs_of_map_2 with "Hmap") as "(?&?)"; eauto; iFrame. }
+    { (* Failure (contradiction) *)
+      incrementPC_inv; simplify_map_eq; eauto. congruence. }
   Qed.
 
   Lemma wp_move_success_reg_fromPC E pc_p pc_g pc_b pc_e pc_a pc_a' w r1 wr1 pc_p' :
@@ -399,394 +254,27 @@ Section cap_lang_rules.
     PC ≠ r1 →
 
     {{{ ▷ PC ↦ᵣ inr ((pc_p,pc_g),pc_b,pc_e,pc_a)
-          ∗ ▷ pc_a ↦ₐ[pc_p'] w
-          ∗ ▷ r1 ↦ᵣ wr1 }}}
+        ∗ ▷ pc_a ↦ₐ[pc_p'] w
+        ∗ ▷ r1 ↦ᵣ wr1 }}}
       Instr Executable @ E
       {{{ RET NextIV;
           PC ↦ᵣ inr ((pc_p,pc_g),pc_b,pc_e,pc_a')
-             ∗ pc_a ↦ₐ[pc_p'] w
-             ∗ r1 ↦ᵣ inr ((pc_p,pc_g),pc_b,pc_e,pc_a) }}}.
+          ∗ pc_a ↦ₐ[pc_p'] w
+          ∗ r1 ↦ᵣ inr ((pc_p,pc_g),pc_b,pc_e,pc_a) }}}.
   Proof.
-    iIntros (Hinstr Hfl Hvpc Hpca' Hne ϕ) "(>HPC & >Hpc_a & >Hr1) Hϕ".
-    iApply wp_lift_atomic_head_step_no_fork; auto.
-    iIntros (σ1 l1 l2 n) "Hσ1 /=". destruct σ1; simpl.
-    iDestruct "Hσ1" as "[Hr Hm]".
-    assert (pc_p' ≠ O).
-    { destruct pc_p'; auto. destruct pc_p; inversion Hfl. inversion Hvpc; subst;
-      destruct H7 as [Hcontr | [Hcontr | Hcontr]]; inversion Hcontr. }
-    iDestruct (@gen_heap_valid with "Hr HPC") as %?.
-    iDestruct (@gen_heap_valid_cap with "Hm Hpc_a") as %?; auto. 
-    iDestruct (@gen_heap_valid with "Hr Hr1") as %?.
-    option_locate_mr m r.
-    assert (<[r1:=inr ((pc_p,pc_g),pc_b,pc_e,pc_a)]> r !r! PC = (inr (pc_p, pc_g, pc_b, pc_e, pc_a)))
-      as Hpc_new1.
-    { rewrite (locate_ne_reg _ _ _ (inr (pc_p, pc_g, pc_b, pc_e, pc_a))); eauto. } 
-    iApply fupd_frame_l.
-    iSplit.
-    - rewrite /reducible.
-      iExists [], (Instr _),(updatePC (update_reg (r,m) r1 (inr ((pc_p,pc_g),pc_b,pc_e,pc_a)))).2, [].
-      iPureIntro.
-      constructor.
-      apply (step_exec_instr (r,m) pc_p pc_g pc_b pc_e pc_a
-                             (Mov r1 (inr PC))
-                             (NextI,_)); eauto; simpl; try congruence.
-        by rewrite /updatePC /update_reg /= HPC Hpc_new1 Hpca' /=.  
-    - (*iMod (fupd_intro_mask' ⊤) as "H"; eauto.*)
-      iModIntro. iNext.
-      iIntros (e1 σ2 efs Hstep).
-      inv_head_step_advanced m r HPC Hpc_a Hinstr Hstep Hpc_new1.
-      rewrite /updatePC /update_reg /= HPC Hpc_new1 Hpca' /=.  
-      iMod (@gen_heap_update with "Hr Hr1") as "[Hr Hr1]". 
-      iMod (@gen_heap_update with "Hr HPC") as "[$ HPC]". 
-      iSpecialize ("Hϕ" with "[HPC Hr1 Hpc_a]"); iFrame; eauto.
-  Qed.
+    iIntros (Hinstr Hfl Hvpc Hpca' Hne ϕ) "(>HPC & >Hpc_a & >Hr1) Hφ".
+    iDestruct (map_of_regs_2 with "HPC Hr1") as "[Hmap %]".
+    iApply (wp_Mov with "[$Hmap Hpc_a]"); eauto; simplify_map_eq; eauto.
+    by unfold regs_of; rewrite !dom_insert; set_solver+.
+    iNext. iIntros (regs' retv) "(#Hspec & Hpc_a & Hmap)". iDestruct "Hspec" as %Hspec.
 
-  Lemma wp_move_fail_z E pc_p pc_g pc_b pc_e pc_a w r1 wr1 z pc_p' :
-    cap_lang.decode w = Mov r1 (inl z) →
-    PermFlows pc_p pc_p' →
-    isCorrectPC (inr ((pc_p,pc_g),pc_b,pc_e,pc_a)) →
-    (pc_a + 1)%a = None →
-    PC ≠ r1 →
-
-    {{{ ▷ PC ↦ᵣ inr ((pc_p,pc_g),pc_b,pc_e,pc_a)
-          ∗ ▷ pc_a ↦ₐ[pc_p'] w
-          ∗ ▷ r1 ↦ᵣ wr1 }}}
-      Instr Executable @ E
-      {{{ RET FailedV;
-          PC ↦ᵣ inr ((pc_p,pc_g),pc_b,pc_e,pc_a)
-             ∗ pc_a ↦ₐ[pc_p'] w
-             ∗ r1 ↦ᵣ inl z }}}.
-  Proof.
-    iIntros (Hinstr Hfl Hvpc Hpca' Hne ϕ) "(>HPC & >Hpc_a & >Hr1) Hϕ".
-    iApply wp_lift_atomic_head_step_no_fork; auto.
-    iIntros (σ1 l1 l2 n) "Hσ1 /=". destruct σ1; simpl.
-    iDestruct "Hσ1" as "[Hr Hm]".
-    assert (pc_p' ≠ O).
-    { destruct pc_p'; auto. destruct pc_p; inversion Hfl. inversion Hvpc; subst;
-      destruct H7 as [Hcontr | [Hcontr | Hcontr]]; inversion Hcontr. }
-    iDestruct (@gen_heap_valid with "Hr HPC") as %?.
-    iDestruct (@gen_heap_valid_cap with "Hm Hpc_a") as %?; auto. 
-    iDestruct (@gen_heap_valid with "Hr Hr1") as %?.
-    option_locate_mr m r.
-    assert (<[r1:=inl z]> r !r! PC = (inr (pc_p, pc_g, pc_b, pc_e, pc_a)))
-      as Hpc_new1.
-    { rewrite (locate_ne_reg _ _ _ (inr (pc_p, pc_g, pc_b, pc_e, pc_a))); eauto. } 
-    iApply fupd_frame_l.
-    iSplit.
-    - rewrite /reducible.
-      iExists [], (Instr _),_, [].
-      iPureIntro.
-      constructor.
-      eapply (step_exec_instr (r,m) pc_p pc_g pc_b pc_e pc_a
-                              (Mov r1 (inl z))
-                              (_,_)); eauto; simpl; try congruence.
-        by rewrite /updatePC /update_reg /= Hpc_new1 Hpca'.  
-    - (*iMod (fupd_intro_mask' ⊤) as "H"; eauto.*)
-      iModIntro. iNext.
-      iIntros (e1 σ2 efs Hstep).
-      inv_head_step_advanced m r HPC Hpc_a Hinstr Hstep Hpc_new1.
-      rewrite /updatePC /update_reg /= Hpc_new1 Hpca' /=.  
-      iMod (@gen_heap_update with "Hr Hr1") as "[Hr Hr1]". 
-      iSpecialize ("Hϕ" with "[HPC Hr1 Hpc_a]"); iFrame; eauto.
-  Qed.
-
-  Lemma wp_move_fail_reg E pc_p pc_g pc_b pc_e pc_a w r1 wr1 rv wrv pc_p' :
-    cap_lang.decode w = Mov r1 (inr rv) →
-    PermFlows pc_p pc_p' →
-    isCorrectPC (inr ((pc_p,pc_g),pc_b,pc_e,pc_a)) →
-    (pc_a + 1)%a = None →
-    PC ≠ r1 →
-
-    {{{ ▷ PC ↦ᵣ inr ((pc_p,pc_g),pc_b,pc_e,pc_a)
-          ∗ ▷ pc_a ↦ₐ[pc_p'] w
-          ∗ ▷ r1 ↦ᵣ wr1
-          ∗ ▷ rv ↦ᵣ wrv }}}
-      Instr Executable @ E
-      {{{ RET FailedV;
-          PC ↦ᵣ inr ((pc_p,pc_g),pc_b,pc_e,pc_a)
-             ∗ pc_a ↦ₐ[pc_p'] w
-             ∗ r1 ↦ᵣ wrv
-             ∗ rv ↦ᵣ wrv }}}.
-  Proof.
-    iIntros (Hinstr Hfl Hvpc Hpca' Hne ϕ) "(>HPC & >Hpc_a & >Hr1 & >Hrv) Hϕ".
-    iApply wp_lift_atomic_head_step_no_fork; auto.
-    iIntros (σ1 l1 l2 n) "Hσ1 /=". destruct σ1; simpl.
-    iDestruct "Hσ1" as "[Hr Hm]".
-    assert (pc_p' ≠ O).
-    { destruct pc_p'; auto. destruct pc_p; inversion Hfl. inversion Hvpc; subst;
-      destruct H7 as [Hcontr | [Hcontr | Hcontr]]; inversion Hcontr. }
-    iDestruct (@gen_heap_valid with "Hr HPC") as %?.
-    iDestruct (@gen_heap_valid_cap with "Hm Hpc_a") as %?; auto. 
-    iDestruct (@gen_heap_valid with "Hr Hr1") as %?.
-    iDestruct (@gen_heap_valid with "Hr Hrv") as %?.
-    option_locate_mr m r.
-    assert (<[r1:=wrv]> r !r! PC = (inr (pc_p, pc_g, pc_b, pc_e, pc_a)))
-      as Hpc_new1.
-    { rewrite (locate_ne_reg _ _ _ (inr (pc_p, pc_g, pc_b, pc_e, pc_a))); eauto. } 
-    iApply fupd_frame_l.
-    iSplit.
-    - rewrite /reducible.
-      iExists [], (Instr _),_, [].
-      iPureIntro.
-      constructor.
-      eapply (step_exec_instr (r,m) pc_p pc_g pc_b pc_e pc_a
-                              (Mov r1 (inr rv))
-                              (_,_)); eauto; simpl; try congruence.
-        by rewrite /updatePC /update_reg /= Hrv Hpc_new1 Hpca'.  
-    - (*iMod (fupd_intro_mask' ⊤) as "H"; eauto.*)
-      iModIntro. iNext.
-      iIntros (e1 σ2 efs Hstep).
-      inv_head_step_advanced m r HPC Hpc_a Hinstr Hstep Hpc_new1.
-      rewrite /updatePC /update_reg /= Hrv Hpc_new1 Hpca' /=.  
-      iMod (@gen_heap_update with "Hr Hr1") as "[Hr Hr1]".
-      iSpecialize ("Hϕ" with "[HPC Hr1 Hpc_a Hrv]"); iFrame; eauto.
-  Qed.
-
-  Lemma wp_move_fail_reg_same E pc_p pc_g pc_b pc_e pc_a w r1 wr1 pc_p' :
-    cap_lang.decode w = Mov r1 (inr r1) →
-    PermFlows pc_p pc_p' →
-    isCorrectPC (inr ((pc_p,pc_g),pc_b,pc_e,pc_a)) →
-    (pc_a + 1)%a = None →
-    PC ≠ r1 →
-
-    {{{ ▷ PC ↦ᵣ inr ((pc_p,pc_g),pc_b,pc_e,pc_a)
-          ∗ ▷ pc_a ↦ₐ[pc_p'] w
-          ∗ ▷ r1 ↦ᵣ wr1 }}}
-      Instr Executable @ E
-      {{{ RET FailedV;
-          PC ↦ᵣ inr ((pc_p,pc_g),pc_b,pc_e,pc_a)
-             ∗ pc_a ↦ₐ[pc_p'] w
-             ∗ r1 ↦ᵣ wr1 }}}.
-  Proof.
-    iIntros (Hinstr Hfl Hvpc Hpca' Hne ϕ) "(>HPC & >Hpc_a & >Hr1) Hϕ".
-    iApply wp_lift_atomic_head_step_no_fork; auto.
-    iIntros (σ1 l1 l2 n) "Hσ1 /=". destruct σ1; simpl.
-    iDestruct "Hσ1" as "[Hr Hm]".
-    assert (pc_p' ≠ O).
-    { destruct pc_p'; auto. destruct pc_p; inversion Hfl. inversion Hvpc; subst;
-      destruct H7 as [Hcontr | [Hcontr | Hcontr]]; inversion Hcontr. }
-    iDestruct (@gen_heap_valid with "Hr HPC") as %?.
-    iDestruct (@gen_heap_valid_cap with "Hm Hpc_a") as %?; auto. 
-    iDestruct (@gen_heap_valid with "Hr Hr1") as %?.
-    option_locate_mr m r.
-    assert (<[r1:=wr1]> r !r! PC = (inr (pc_p, pc_g, pc_b, pc_e, pc_a)))
-      as Hpc_new1.
-    { rewrite (locate_ne_reg _ _ _ (inr (pc_p, pc_g, pc_b, pc_e, pc_a))); eauto. } 
-    iApply fupd_frame_l.
-    iSplit.
-    - rewrite /reducible.
-      iExists [], (Instr _),_, [].
-      iPureIntro.
-      constructor.
-      eapply (step_exec_instr (r,m) pc_p pc_g pc_b pc_e pc_a
-                              (Mov r1 (inr r1))
-                              (_,_)); eauto; simpl; try congruence.
-        by rewrite /updatePC /update_reg /= Hr1 Hpc_new1 Hpca'.  
-    - (*iMod (fupd_intro_mask' ⊤) as "H"; eauto.*)
-      iModIntro. iNext.
-      iIntros (e1 σ2 efs Hstep).
-      inv_head_step_advanced m r HPC Hpc_a Hinstr Hstep Hpc_new1.
-      rewrite /updatePC /update_reg /= Hr1 Hpc_new1 Hpca' /=.  
-      iMod (@gen_heap_update with "Hr Hr1") as "[Hr Hr1]". 
-      iSpecialize ("Hϕ" with "[HPC Hr1 Hpc_a]"); iFrame; eauto.
-  Qed.
-
-  Lemma wp_move_fail_reg_samePC E pc_p pc_g pc_b pc_e pc_a w pc_p' :
-    cap_lang.decode w = Mov PC (inr PC) →
-    PermFlows pc_p pc_p' →
-    isCorrectPC (inr ((pc_p,pc_g),pc_b,pc_e,pc_a)) →
-    (pc_a + 1)%a = None →
-
-    {{{ ▷ PC ↦ᵣ inr ((pc_p,pc_g),pc_b,pc_e,pc_a)
-          ∗ ▷ pc_a ↦ₐ[pc_p'] w }}}
-      Instr Executable @ E
-      {{{ RET FailedV;
-          PC ↦ᵣ inr ((pc_p,pc_g),pc_b,pc_e,pc_a)
-             ∗ pc_a ↦ₐ[pc_p'] w }}}.
-  Proof.
-    iIntros (Hinstr Hfl Hvpc Hpca' ϕ) "(>HPC & >Hpc_a) Hϕ".
-    iApply wp_lift_atomic_head_step_no_fork; auto.
-    iIntros (σ1 l1 l2 n) "Hσ1 /=". destruct σ1; simpl.
-    iDestruct "Hσ1" as "[Hr Hm]".
-    assert (pc_p' ≠ O).
-    { destruct pc_p'; auto. destruct pc_p; inversion Hfl. inversion Hvpc; subst;
-      destruct H7 as [Hcontr | [Hcontr | Hcontr]]; inversion Hcontr. }
-    iDestruct (@gen_heap_valid with "Hr HPC") as %?.
-    iDestruct (@gen_heap_valid_cap with "Hm Hpc_a") as %?; auto. 
-    option_locate_mr m r.
-    iApply fupd_frame_l.
-    iSplit.
-    - rewrite /reducible.
-      iExists [], (Instr _),_, [].
-      iPureIntro.
-      constructor.
-      eapply (step_exec_instr (r,m) pc_p pc_g pc_b pc_e pc_a
-                              (Mov PC (inr PC))
-                              (_,_)); eauto; simpl; try congruence.
-      rewrite /updatePC /update_reg /= /RegLocate lookup_insert.
-      rewrite /RegLocate in HPC. rewrite HPC Hpca'. eauto.
-    - (*iMod (fupd_intro_mask' ⊤) as "H"; eauto.*)
-      iModIntro. iNext.
-      iIntros (e1 σ2 efs Hstep).
-      inv_head_step_advanced m r HPC Hpc_a Hinstr Hstep HPC.
-      rewrite /updatePC /update_reg /= /RegLocate lookup_insert.
-      rewrite /RegLocate in HPC. rewrite HPC Hpca' /=.
-      iMod (@gen_heap_update with "Hr HPC") as "[$ HPC]".
-      iSpecialize ("Hϕ" with "[HPC Hpc_a]"); iFrame; eauto.
-  Qed.
-
-  Lemma wp_move_fail_reg_toPC E pc_p pc_g pc_b pc_e pc_a w r1 p g b e a pc_p' :
-    cap_lang.decode w = Mov PC (inr r1) →
-    PermFlows pc_p pc_p' →
-    isCorrectPC (inr ((pc_p,pc_g),pc_b,pc_e,pc_a)) →
-    (a + 1)%a = None →
-
-    {{{ ▷ PC ↦ᵣ inr ((pc_p,pc_g),pc_b,pc_e,pc_a)
-          ∗ ▷ pc_a ↦ₐ[pc_p'] w
-          ∗ ▷ r1 ↦ᵣ inr ((p,g),b,e,a) }}}
-      Instr Executable @ E
-      {{{ RET FailedV;
-          PC ↦ᵣ inr ((p,g),b,e,a)
-             ∗ pc_a ↦ₐ[pc_p'] w
-             ∗ r1 ↦ᵣ inr ((p,g),b,e,a) }}}.
-  Proof.
-    iIntros (Hinstr Hfl Hvpc Hpca' ϕ) "(>HPC & >Hpc_a & >Hr1) Hϕ".
-    iApply wp_lift_atomic_head_step_no_fork; auto.
-    iIntros (σ1 l1 l2 n) "Hσ1 /=". destruct σ1; simpl.
-    iDestruct "Hσ1" as "[Hr Hm]".
-    assert (pc_p' ≠ O).
-    { destruct pc_p'; auto. destruct pc_p; inversion Hfl. inversion Hvpc; subst;
-      destruct H7 as [Hcontr | [Hcontr | Hcontr]]; inversion Hcontr. }
-    iDestruct (@gen_heap_valid with "Hr HPC") as %?.
-    iDestruct (@gen_heap_valid_cap with "Hm Hpc_a") as %?; auto. 
-    iDestruct (@gen_heap_valid with "Hr Hr1") as %?.
-    option_locate_mr m r.
-    iApply fupd_frame_l.
-    iSplit.
-    - rewrite /reducible.
-      iExists [], (Instr _),_, [].
-      iPureIntro.
-      constructor.
-      eapply (step_exec_instr (r,m) pc_p pc_g pc_b pc_e pc_a
-                              (Mov PC (inr r1))
-                              (_,_)); eauto; simpl; try congruence.
-        by rewrite /updatePC /update_reg /= Hr1 /RegLocate lookup_insert Hpca'.
-    - (*iMod (fupd_intro_mask' ⊤) as "H"; eauto.*)
-      iModIntro. iNext.
-      iIntros (e1 σ2 efs Hstep).
-      inv_head_step_advanced m r HPC Hpc_a Hinstr Hstep Hpc_new1.
-      rewrite /updatePC /update_reg /= Hr1 /RegLocate lookup_insert Hpca' /=.
-      iMod (@gen_heap_update with "Hr HPC") as "[$ HPC]".
-      iSpecialize ("Hϕ" with "[HPC Hr1 Hpc_a]"); iFrame; eauto.
-  Qed.
-
-  Lemma wp_move_fail_reg_toPC2 E pc_p pc_g pc_b pc_e pc_a w nr1 z pc_p' :
-    cap_lang.decode w = Mov PC nr1 →
-    PermFlows pc_p pc_p' →
-    isCorrectPC (inr ((pc_p,pc_g),pc_b,pc_e,pc_a)) →
-
-    {{{ ▷ PC ↦ᵣ inr ((pc_p,pc_g),pc_b,pc_e,pc_a)
-          ∗ ▷ pc_a ↦ₐ[pc_p'] w
-          ∗ (match nr1 with inr r1 => (r1 ↦ᵣ inl z) | inl m => ⌜m = z⌝ end) }}}
-      Instr Executable @ E
-      {{{ RET FailedV;
-          PC ↦ᵣ inl z
-             ∗ pc_a ↦ₐ[pc_p'] w
-             ∗ (match nr1 with inr r1 => r1 ↦ᵣ inl z | inl m => ⌜m = z⌝ end) }}}.
-  Proof.
-    iIntros (Hinstr Hfl Hvpc ϕ) "(>HPC & >Hpc_a & Hr1) Hϕ".
-    iApply wp_lift_atomic_head_step_no_fork; auto.
-    iIntros (σ1 l1 l2 n) "Hσ1 /=". destruct σ1; simpl.
-    iDestruct "Hσ1" as "[Hr Hm]".
-    assert (pc_p' ≠ O).
-    { destruct pc_p'; auto. destruct pc_p; inversion Hfl. inversion Hvpc; subst;
-      destruct H7 as [Hcontr | [Hcontr | Hcontr]]; inversion Hcontr. }
-    iDestruct (@gen_heap_valid with "Hr HPC") as %?.
-    iDestruct (@gen_heap_valid_cap with "Hm Hpc_a") as %?; auto. 
-    iAssert (⌜match nr1 with inl m => m = z | inr r1 => r !! r1 = Some (inl z) end⌝)%I with "[Hr Hr1]" as %?.
-    { destruct nr1; auto.
-      iDestruct (@gen_heap_valid with "Hr Hr1") as %?. auto. }
-    option_locate_mr m r.
-    iApply fupd_frame_l.
-    iSplit.
-    - rewrite /reducible. destruct nr1.
-      { iExists [], (Instr _),_, [].
-        iPureIntro.
-        constructor.
-        eapply (step_exec_instr (r,m) pc_p pc_g pc_b pc_e pc_a
-                                (Mov PC _)
-                                (_,_)); eauto; simpl; try congruence.
-        rewrite Hpc_a. eauto.
-        rewrite /updatePC /update_reg /= /RegLocate lookup_insert; eauto. }
-      { iExists [], (Instr _),_, [].
-        iPureIntro.
-        constructor.
-        eapply (step_exec_instr (r,m) pc_p pc_g pc_b pc_e pc_a
-                                (Mov PC _)
-                                (_,_)); eauto; simpl; try congruence.
-        rewrite Hpc_a. eauto.
-        rewrite /updatePC /update_reg /= /RegLocate lookup_insert H4; eauto. }
-    - (*iMod (fupd_intro_mask' ⊤) as "H"; eauto.*)
-      iModIntro. iNext.
-      iIntros (e1 σ2 efs Hstep).
-      inv_head_step_advanced m r HPC Hpc_a Hinstr Hstep Hpc_new1.
-      rewrite /updatePC /update_reg /= /RegLocate.
-      destruct nr1.
-      { rewrite lookup_insert /=. subst z0.
-        iMod (@gen_heap_update with "Hr HPC") as "[$ HPC]".
-        iSpecialize ("Hϕ" with "[HPC Hpc_a]"); iFrame; eauto. }
-      { rewrite lookup_insert /= H4.
-        iMod (@gen_heap_update with "Hr HPC") as "[$ HPC]".
-        iSpecialize ("Hϕ" with "[HPC Hr1 Hpc_a]"); iFrame; eauto. }
-  Qed.
-
-  Lemma wp_move_fail_reg_fromPC E pc_p pc_g pc_b pc_e pc_a w r1 wr1 pc_p' :
-    cap_lang.decode w = Mov r1 (inr PC) →
-    PermFlows pc_p pc_p' →
-    isCorrectPC (inr ((pc_p,pc_g),pc_b,pc_e,pc_a)) →
-    (pc_a + 1)%a = None →
-    PC ≠ r1 →
-
-    {{{ ▷ PC ↦ᵣ inr ((pc_p,pc_g),pc_b,pc_e,pc_a)
-          ∗ ▷ pc_a ↦ₐ[pc_p'] w
-          ∗ ▷ r1 ↦ᵣ wr1 }}}
-      Instr Executable @ E
-      {{{ RET FailedV;
-          PC ↦ᵣ inr ((pc_p,pc_g),pc_b,pc_e,pc_a)
-             ∗ pc_a ↦ₐ[pc_p'] w
-             ∗ r1 ↦ᵣ inr ((pc_p,pc_g),pc_b,pc_e,pc_a) }}}.
-  Proof.
-    iIntros (Hinstr Hfl Hvpc Hpca' Hne ϕ) "(>HPC & >Hpc_a & >Hr1) Hϕ".
-    iApply wp_lift_atomic_head_step_no_fork; auto.
-    iIntros (σ1 l1 l2 n) "Hσ1 /=". destruct σ1; simpl.
-    iDestruct "Hσ1" as "[Hr Hm]".
-    assert (pc_p' ≠ O).
-    { destruct pc_p'; auto. destruct pc_p; inversion Hfl. inversion Hvpc; subst;
-      destruct H7 as [Hcontr | [Hcontr | Hcontr]]; inversion Hcontr. }
-    iDestruct (@gen_heap_valid with "Hr HPC") as %?.
-    iDestruct (@gen_heap_valid_cap with "Hm Hpc_a") as %?; auto. 
-    iDestruct (@gen_heap_valid with "Hr Hr1") as %?.
-    option_locate_mr m r.
-    assert (<[r1:=inr ((pc_p,pc_g),pc_b,pc_e,pc_a)]> r !r! PC = (inr (pc_p, pc_g, pc_b, pc_e, pc_a)))
-      as Hpc_new1.
-    { rewrite (locate_ne_reg _ _ _ (inr (pc_p, pc_g, pc_b, pc_e, pc_a))); eauto. } 
-    iApply fupd_frame_l.
-    iSplit.
-    - rewrite /reducible.
-      iExists [], (Instr _),(updatePC (update_reg (r,m) r1 (inr ((pc_p,pc_g),pc_b,pc_e,pc_a)))).2, [].
-      iPureIntro.
-      constructor.
-      eapply (step_exec_instr (r,m) pc_p pc_g pc_b pc_e pc_a
-                              (Mov r1 (inr PC))
-                              (_,_)); eauto; simpl; try congruence.
-        by rewrite /updatePC /update_reg /= HPC Hpc_new1 Hpca' /=.  
-    - (*iMod (fupd_intro_mask' ⊤) as "H"; eauto.*)
-      iModIntro. iNext.
-      iIntros (e1 σ2 efs Hstep).
-      inv_head_step_advanced m r HPC Hpc_a Hinstr Hstep Hpc_new1.
-      rewrite /updatePC /update_reg /= HPC Hpc_new1 Hpca' /=.  
-      iMod (@gen_heap_update with "Hr Hr1") as "[Hr Hr1]". 
-      iSpecialize ("Hϕ" with "[HPC Hr1 Hpc_a]"); iFrame; eauto.
+    destruct Hspec as [|].
+    { (* Success *)
+      iApply "Hφ". iFrame. incrementPC_inv; simplify_map_eq.
+      rewrite (insert_commute _ PC r1) // insert_insert insert_commute // insert_insert.
+      iDestruct (regs_of_map_2 with "Hmap") as "(?&?)"; eauto; iFrame. }
+    { (* Failure (contradiction) *)
+      incrementPC_inv; simplify_map_eq; eauto. congruence. }
   Qed.
 
 End cap_lang_rules.
